Added comp_gmap

interface/Polymorphic_gmap.fsti
@@ -1,43 +1,53 @@
 module Polymorphic_gmap
 
-(*module M = Dependent_map
+module M = Dependent_map
 open FStar.Seq
-module S =  Set_extended
+module S = FStar.Set //Set_extended
 
-//key type
-type key_t =
-  |Alpha_t
-  |Beta_t
+type kt : eqtype =
+  |Alpha_t : string -> kt
+  |Beta_t : string -> kt
 
-val concrete_st_a : eqtype
+//concrete state of alpha type
+val concrete_st_a : Type0
 
-val concrete_st_b : eqtype
+//concrete state of beta type
+val concrete_st_b : Type0
 
-type kt = string & key_t
-
-//value type
-let vt (c:key_t) : eqtype = 
+let vt (c:kt) : Type0 =
   match c with
-  | Alpha_t -> concrete_st_a
-  | Beta_t -> concrete_st_b
+  |Alpha_t _ -> concrete_st_a
+  |Beta_t _ -> concrete_st_b
 
-type concrete_st = M.t kt (fun (_,t) -> vt t)
+//concrete state
+type concrete_st = M.t kt vt
 
-val init_st_a : concrete_st_a
+//init state of alpha type
+val init_st_a : concrete_st_a 
 
+//init state of beta type
 val init_st_b : concrete_st_b
 
-let init_st_v (c:key_t) : vt c =
-  match c with
-  |Alpha_t -> init_st_a
-  |Beta_t -> init_st_b
+let init_st_v (k:kt) : vt k =
+  match k with
+  |Alpha_t _ -> init_st_a
+  |Beta_t _ -> init_st_b
 
-let sel (s:concrete_st) (k:kt) : vt (snd k)  =
-    if M.contains s k then M.sel s k else (init_st_v (snd k))
-    
+let init_st (k:kt) : concrete_st = M.const_on S.empty (fun k -> init_st_v k)
+
+//Querying the map for its value at a given key
+let sel (s:concrete_st) (k:kt) =
+  match k with
+  |Alpha_t _ -> if M.contains s k then M.sel s k else init_st_a
+  |Beta_t _ -> if M.contains s k then M.sel s k else init_st_b
+
+let eq_a (a b:concrete_st_a) = a == b
+
+let eq_b (a b:concrete_st_b) = a == b
+
 let eq (a b:concrete_st) =
-  M.equal a b //(forall k t. M.contains a (k,t) = M.contains b (k,t)) /\
-  //(forall k t. M.contains a (k,t) ==> M.sel a (k,t) == M.sel b (k,t))
+  //M.equal a b
+  (forall k. M.contains a k = M.contains b k /\ sel a k == sel b k)
 
 let symmetric (a b:concrete_st) 
   : Lemma (requires eq a b)
@@ -51,32 +61,37 @@ let eq_is_equiv (a b:concrete_st)
   : Lemma (requires a == b)
           (ensures eq a b) = ()
 
+//alpha MRDT operation type
 val app_op_a : eqtype
 
+//beta MRDT operation type
 val app_op_b : eqtype
-  
+
 type app_op_v : eqtype =
   |Alpha_op : app_op_a -> app_op_v
   |Beta_op : app_op_b -> app_op_v
 
-//operation type
 type app_op_t:eqtype =
   |Set : string (* key *) -> app_op_v (* value op *) -> app_op_t
-  
+
 type op_t = pos (*timestamp*) & (nat (*replica ID*) & app_op_t)
-
 type op_v = pos (*timestamp*) & (nat (*replica ID*) & app_op_v)
-
 type op_a = pos (*timestamp*) & (nat (*replica ID*) & app_op_a)
-
 type op_b = pos (*timestamp*) & (nat (*replica ID*) & app_op_b)
+
+let get_rid (_,(rid,_)) = rid
+
+let distinct_ops (ts1,_) (ts2,_) = ts1 =!= ts2
 
 let is_alpha_op (o:op_t) =
   match snd (snd o) with
   |Set _ (Alpha_op _) -> true
   |_ -> false
 
-let is_beta_op (o:op_t) = not (is_alpha_op o)
+let is_beta_op (o:op_t) = 
+  match snd (snd o) with
+  |Set _ (Beta_op _) -> true
+  |_ -> false
   
 let get_op_a (o:op_t{is_alpha_op o}) : op_a =
   match o with
@@ -85,30 +100,22 @@ let get_op_a (o:op_t{is_alpha_op o}) : op_a =
 let get_op_b (o:op_t{~ (is_alpha_op o)}) : op_b =
   match o with
   |ts, (rid, Set _ (Beta_op op)) -> (ts,(rid,op))
-
+  
+//do function of alpha type
 val do_a (s:concrete_st_a) (o:op_a) : concrete_st_a
 
+//do function of beta type
 val do_b (s:concrete_st_b) (o:op_b) : concrete_st_b
 
-(*let do_v (s:concrete_st_v) (o:op_t{(Alpha? s <==> is_alpha_op o) /\ (Beta? s <==> is_beta_op o)}) : concrete_st_v =
-  if is_alpha_op o then
-    let Alpha c = s in Alpha (do_a c (get_op_a o))
-  else let Beta c = s in Beta (do_b c (get_op_b o))*)
-
-let get_rid (_,(rid,_)) = rid
-
-let distinct_ops (ts1,_) (ts2,_) = ts1 =!= ts2
-
-let get_op_v (o:op_t) : op_v =
-  match o with
-  |(ts,(rid,(Set k op))) -> (ts,(rid,op))
-
-let do (s:concrete_st) (o:op_t(*{do_pre s o}*)) : concrete_st =
-  match o with
-    |_,(_,Set k (Alpha_op _)) -> M.upd s (k,Alpha_t) (do_a (sel s (k,Alpha_t)) (get_op_a o))
-    |_,(_,Set k (Beta_op _)) -> M.upd s (k,Beta_t) (do_b (sel s (k,Beta_t)) (get_op_b o))
-
 let get_key (_,(_,Set k _)) = k
+
+//do function of map
+let do (s:concrete_st) (o:op_t) 
+  : (r:concrete_st{(is_alpha_op o ==> (forall k. M.contains r k <==> M.contains s k \/ k = Alpha_t (get_key o))) /\
+                   (is_beta_op o ==> (forall k. M.contains r k <==> M.contains s k \/ k = Beta_t (get_key o)))}) =
+  match snd (snd o) with
+  |Set k (Alpha_op _) -> let v = sel s (Alpha_t k) in M.upd s (Alpha_t k) (do_a v (get_op_a o))
+  |Set k (Beta_op _) -> let v = sel s (Beta_t k) in M.upd s (Beta_t k) (do_b v (get_op_b o))
 
 type rc_res =
   |Fst_then_snd //o1 -> o2
@@ -130,216 +137,16 @@ val merge_a (l a b:concrete_st_a) : concrete_st_a
 
 val merge_b (l a b:concrete_st_b) : concrete_st_b
 
-#set-options "--query_stats"
-// concrete merge operation
-let merge (l a b:concrete_st) : concrete_st =
-  let (keys:S.t kt) = S.union (M.domain l) (S.union (M.domain a) (M.domain b)) in
-  let u = M.const_on keys (fun kt -> init_st_v (snd kt)) in
-  M.iter_upd (fun kt _ -> (if snd kt = Alpha_t then (merge_a (sel l kt) (sel a kt) (sel b kt))
-                           else (merge_b (sel l kt) (sel a kt) (sel b kt)))) u 
-
-let commutes_with (o1 o2:op_t) =
-  forall s. eq (do (do s o1) o2) (do (do s o2) o1)
-
-type log = seq op_t
-
-// applying a log of operations to a concrete state
-let rec apply_log (x:concrete_st) (l:log) : Tot concrete_st (decreases length l) =
-  match length l with
-  |0 -> x
-  |_ -> apply_log (do x (head l)) (tail l)  *)
-
-module S = Set_extended
-module M = Map_extended
-open FStar.Seq
-
-//key type
-type key_t =
-  |Alpha_t
-  |Beta_t
-
-val concrete_st_a : Type0
-
-val concrete_st_b : Type0
-
-// concrete state of values
-noeq type concrete_st_v = 
-  |Alpha : concrete_st_a -> concrete_st_v
-  |Beta : concrete_st_b -> concrete_st_v
-
-let eq_key_t (s:M.t (string & key_t) concrete_st_v) =
-  (forall sk. M.contains s sk ==> (let v = M.sel s sk in
-         ((Alpha? v <==> snd sk == Alpha_t) /\ (Beta? v <==> snd sk = Beta_t))))
-
-//concrete state
-let concrete_st = s:M.t (string & key_t) concrete_st_v {eq_key_t s}
-
-val init_st_a : concrete_st_a
-
-val init_st_b : concrete_st_b
-
-let init_st_v (t:key_t) : concrete_st_v =
-  match t with
-  |Alpha_t -> Alpha init_st_a
-  |Beta_t -> Beta init_st_b
-
-let init_st (t:key_t) : concrete_st = M.const_on S.empty (init_st_v t)
-
-let geta (s:concrete_st_v{Alpha? s}) =
-  let Alpha x = s in x
-
-let getb (s:concrete_st_v{Beta? s}) =
-  let Beta x = s in x
-
-let sel_a (s:concrete_st) k  =
-    if M.contains s (k,Alpha_t) then geta (M.sel s (k,Alpha_t)) else init_st_a
-
-let sel_b (s:concrete_st) k  =
-    if M.contains s (k,Beta_t) then getb (M.sel s (k,Beta_t)) else init_st_b
-
-let eq_a (a b:concrete_st_a) : Type0 = a == b
-
-let eq_b (a b:concrete_st_b) : Type0 = a == b
-
-let eq_v (a:concrete_st_v) (b:concrete_st_v) : Type0 = //{(Ctr? a ==> Ctr? b) /\ (Gset? a ==> Gset? b)}) : Type0 =
-  match a,b with
-  |Alpha x,Alpha y -> eq_a x y
-  |Beta x, Beta y -> eq_b x y
-  |_ -> False
-
-// equivalence relation
-let eq (a b:concrete_st) =
-  (forall k t. M.contains a (k,t) = M.contains b (k,t)) /\
-  (forall k t. M.contains a (k,t) ==> (Alpha_t? t ==> eq_a (sel_a a k) (sel_a b k)) /\
-                                 (Beta_t? t ==> eq_b (sel_b a k) (sel_b b k)))
-
-val symmetric_a (a b:concrete_st_a)
-  : Lemma (requires eq_a a b)
-          (ensures eq_a b a) 
-          [SMTPat (eq_a a b)]
-
-val symmetric_b (a b:concrete_st_b)
-  : Lemma (requires eq_b a b)
-          (ensures eq_b b a) 
-          [SMTPat (eq_b a b)]
-          
-let symmetric (a b:concrete_st) 
-  : Lemma (requires eq a b)
-          (ensures eq b a) = ()
-
-val transitive_a (a b c:concrete_st_a)
-  : Lemma (requires eq_a a b /\ eq_a b c)
-          (ensures eq_a a c)
-          [SMTPat (eq_a a b /\ eq_a b c)]
-
-val transitive_b (a b c:concrete_st_b)
-  : Lemma (requires eq_b a b /\ eq_b b c)
-          (ensures eq_b a c)
-          [SMTPat (eq_b a b /\ eq_b b c)]
-          
-val transitive (a b c:concrete_st)
-  : Lemma (requires eq a b /\ eq b c)
-          (ensures eq a c) 
-
-val eq_is_equiv_a (a b:concrete_st_a)
-  : Lemma (requires a == b)
-          (ensures eq_a a b) 
-          [SMTPat (a == b)]
-
-val eq_is_equiv_b (a b:concrete_st_b)
-  : Lemma (requires a == b)
-          (ensures eq_b a b)
-          [SMTPat (a == b)]
-          
-val eq_is_equiv (a b:concrete_st)
-  : Lemma (requires a == b)
-          (ensures eq a b)
-
-val app_op_a : eqtype
-
-val app_op_b : eqtype
-  
-type app_op_v : eqtype =
-  |Alpha_op : app_op_a -> app_op_v
-  |Beta_op : app_op_b -> app_op_v
-
-//operation type
-type app_op_t:eqtype =
-  |Set : string (* key *) -> app_op_v (* value op *) -> app_op_t
-  
-type op_t = pos (*timestamp*) & (nat (*replica ID*) & app_op_t)
-
-type op_v = pos (*timestamp*) & (nat (*replica ID*) & app_op_v)
-
-type op_a = pos (*timestamp*) & (nat (*replica ID*) & app_op_a)
-
-type op_b = pos (*timestamp*) & (nat (*replica ID*) & app_op_b)
-
-let is_alpha_op (o:op_t) =
-  match snd (snd o) with
-  |Set _ (Alpha_op _) -> true
-  |_ -> false
-
-let is_beta_op (o:op_t) = not (is_alpha_op o)
-  
-let get_op_a (o:op_t{is_alpha_op o}) : op_a =
-  match o with
-  |ts, (rid, Set _ (Alpha_op op)) -> (ts,(rid,op))
-
-let get_op_b (o:op_t{~ (is_alpha_op o)}) : op_b =
-  match o with
-  |ts, (rid, Set _ (Beta_op op)) -> (ts,(rid,op))
-
-val do_a (s:concrete_st_a) (o:op_a) : concrete_st_a
-
-val do_b (s:concrete_st_b) (o:op_b) : concrete_st_b
-
-let do_v (s:concrete_st_v) (o:op_t{(Alpha? s <==> is_alpha_op o) /\ (Beta? s <==> is_beta_op o)}) : concrete_st_v =
-  if is_alpha_op o then
-    let Alpha c = s in Alpha (do_a c (get_op_a o))
-  else let Beta c = s in Beta (do_b c (get_op_b o))
-
-let get_rid (_,(rid,_)) = rid
-
-let distinct_ops (ts1,_) (ts2,_) = ts1 =!= ts2
-
-let get_op_v (o:op_t) : op_v =
-  match o with
-  |(ts,(rid,(Set k op))) -> (ts,(rid,op))
-
-let do (s:concrete_st) (o:op_t(*{do_pre s o}*)) : concrete_st =
-  match o with
-    |_,(_,Set k (Alpha_op _)) -> M.upd s (k,Alpha_t) (do_v (Alpha (sel_a s k)) o)
-    |_,(_,Set k (Beta_op _)) -> M.upd s (k,Beta_t) (do_v (Beta (sel_b s k)) o)
-
-let get_key (_,(_,Set k _)) = k
-
-type rc_res =
-  |Fst_then_snd //o1 -> o2
-  |Snd_then_fst //o2 -> o1
-  |Either
-
-val rc_a (o1 o2:op_a) : rc_res
-
-val rc_b (o1 o2:op_b) : rc_res
-
-//conflict resolution
-let rc (o1 o2:op_t) : rc_res = 
-  match snd (snd o1), snd (snd o2) with
-  |Set k1 (Alpha_op _), Set k2 (Alpha_op _) -> if k1 = k2 then rc_a (get_op_a o1) (get_op_a o2) else Either
-  |Set k1 (Beta_op _), Set k2 (Beta_op _) -> if k1 = k2 then rc_b (get_op_b o1) (get_op_b o2) else Either
-  |_ -> Either
-
-val merge_a (l a b:concrete_st_a) : concrete_st_a 
-
-val merge_b (l a b:concrete_st_b) : concrete_st_b
+let compose_values (k:kt) (l a b:concrete_st) : vt k =
+  if Alpha_t? k then 
+    merge_a (sel l k) (sel a k) (sel b k)
+  else merge_b (sel l k) (sel a k) (sel b k)
 
 // concrete merge operation
 let merge (l a b:concrete_st) : concrete_st =
   let keys = S.union (M.domain l) (S.union (M.domain a) (M.domain b)) in
-  let u = M.const_on keys init_st_a in
-  M.iter_upd (fun (k,t) v -> if Alpha_t? t then Alpha (merge_a (sel_a l k) (sel_a a k) (sel_a b k))
-                          else Beta (merge_b (sel_b l k) (sel_b a k) (sel_b b k))) u
+  let u = M.const_on keys (fun k -> init_st k) in
+  M.iter_upd (fun k _ -> compose_values k l a b) u
 
 let commutes_with_a (o1 o2:op_a) =
   forall s. eq_a (do_a (do_a s o1) o2) (do_a (do_a s o2) o1)
@@ -358,13 +165,12 @@ let rec apply_log (x:concrete_st) (l:log) : Tot concrete_st (decreases length l)
   |0 -> x
   |_ -> apply_log (do x (head l)) (tail l)  
 
-
 /////////////////////////////////////////////////////////////////////////////
 
 val rc_non_comm (o1 o2:op_t)
   : Lemma (requires distinct_ops o1 o2)
-          (ensures Either? (rc o1 o2) <==> commutes_with o1 o2) 
-          
+          (ensures Either? (rc o1 o2) <==> commutes_with o1 o2)
+
 val no_rc_chain (o1 o2 o3:op_t)
   : Lemma (requires distinct_ops o1 o2 /\ distinct_ops o2 o3)
           (ensures ~ (Fst_then_snd? (rc o1 o2) /\ Fst_then_snd? (rc o2 o3)))
@@ -402,7 +208,7 @@ val merge_idem_a (s: concrete_st_a)
 val merge_idem_b (s: concrete_st_b) 
   : Lemma (ensures eq_b (merge_b s s s) s)
           [SMTPat (merge_b s s s)]
-          
+
 let merge_idem (s:concrete_st)
   : Lemma (ensures eq (merge s s s) s) = ()
 
@@ -437,10 +243,11 @@ let rc_ind_right (l a b:concrete_st) (o1 o2 o2':op_t)
                     eq (merge l (do a o1) (do b o2)) (do (merge l (do a o1) b) o2))
           (ensures eq (merge l (do a o1) (do (do b o2') o2)) (do (merge l (do a o1) (do b o2')) o2)) =
   let k = get_key o2' in
+  let ka = Alpha_t k in let kb = Beta_t k in
   if is_alpha_op o2' && is_alpha_op o1 && get_key o2 = k && Fst_then_snd? (rc_a (get_op_a o1) (get_op_a o2)) then
-    rc_ind_right_a (sel_a l k) (sel_a a k) (sel_a b k) (get_op_a o1) (get_op_a o2) (get_op_a o2')
+    rc_ind_right_a (sel l ka) (sel a ka) (sel b ka) (get_op_a o1) (get_op_a o2) (get_op_a o2')
   else if is_beta_op o2' && is_beta_op o1 && get_key o2 = k && Fst_then_snd? (rc_b (get_op_b o1) (get_op_b o2)) then 
-    rc_ind_right_b (sel_b l k) (sel_b a k) (sel_b b k) (get_op_b o1) (get_op_b o2) (get_op_b o2')
+    rc_ind_right_b (sel l kb) (sel a kb) (sel b kb) (get_op_b o1) (get_op_b o2) (get_op_b o2')
   else rc_ind_right_ne l a b o1 o2 o2'
 
 val rc_ind_left_a (l a b:concrete_st_a) (o1 o2 o1':op_a) 
@@ -470,11 +277,13 @@ let rc_ind_left (l a b:concrete_st) (o1 o2 o1':op_t)
                     eq (merge l (do a o1) (do b o2)) (do (merge l (do a o1) b) o2))
           (ensures eq (merge l (do (do a o1') o1) (do b o2)) (do (merge l (do (do a o1') o1) b) o2)) =
   let k = get_key o1' in
+  let ka = Alpha_t k in let kb = Beta_t k in
   if is_alpha_op o1' && is_alpha_op o1 && get_key o2 = k && Fst_then_snd? (rc_a (get_op_a o1) (get_op_a o2)) then
-    rc_ind_left_a (sel_a l k) (sel_a a k) (sel_a b k) (get_op_a o1) (get_op_a o2) (get_op_a o1')
+    rc_ind_left_a (sel l ka) (sel a ka) (sel b ka) (get_op_a o1) (get_op_a o2) (get_op_a o1')
   else if is_beta_op o1' && is_beta_op o1 && get_key o2 = k && Fst_then_snd? (rc_b (get_op_b o1) (get_op_b o2)) then 
-    rc_ind_left_b (sel_b l k) (sel_b a k) (sel_b b k) (get_op_b o1) (get_op_b o2) (get_op_b o1')
+    rc_ind_left_b (sel l kb) (sel a kb) (sel b kb) (get_op_b o1) (get_op_b o2) (get_op_b o1')
   else rc_ind_left_ne l a b o1 o2 o1'
+
 
 val rc_ind_lca_a (l:concrete_st_a) (o1 o2 o:op_a)
   : Lemma (requires Fst_then_snd? (rc_a o1 o2) /\
@@ -495,13 +304,14 @@ let rc_ind_lca (l:concrete_st) (o1 o2 o:op_t)
                     eq (merge l (do l o1) (do l o2)) (do (do l o1) o2))
           (ensures eq (merge (do l o) (do (do l o) o1) (do (do l o) o2)) (do (do (do l o) o1) o2)) =
   let k = get_key o in
+  let ka = Alpha_t k in let kb = Beta_t k in
   if get_key o1 = k && is_alpha_op o1 && is_alpha_op o && Fst_then_snd? (rc_a (get_op_a o1) (get_op_a o2)) then 
-    rc_ind_lca_a (sel_a l k) (get_op_a o1) (get_op_a o2) (get_op_a o)
+    rc_ind_lca_a (sel l ka) (get_op_a o1) (get_op_a o2) (get_op_a o)
   else if get_key o1 = k && is_beta_op o1 && is_beta_op o && Fst_then_snd? (rc_b (get_op_b o1) (get_op_b o2)) then 
-    rc_ind_lca_b (sel_b l k) (get_op_b o1) (get_op_b o2) (get_op_b o)
+    rc_ind_lca_b (sel l kb) (get_op_b o1) (get_op_b o2) (get_op_b o)
   else ()
 
-val rc_base (o1 o2:op_t) (t:key_t)
+val rc_base (o1 o2:op_t) (t:kt)
   : Lemma (requires Fst_then_snd? (rc o1 o2) /\ distinct_ops o1 o2)
           (ensures eq (merge (init_st t) (do (init_st t) o1) (do (init_st t) o2)) (do (do (init_st t) o1) o2))
 
@@ -540,10 +350,11 @@ let rc_inter_base_right (l a b c:concrete_st) (o1 o2 ob ol:op_t)
                     eq (merge l (do a ol) (do b ob)) (do (do c ob) ol)) //***EXTRA***
           (ensures eq (merge (do l ol) (do (do a ol) o1) (do (do (do b ob) ol) o2)) (do (do (do (do c ob) ol) o1) o2)) =
   let k = get_key ob in
+  let ka = Alpha_t k in let kb = Beta_t k in
   if get_key o2 = k && is_alpha_op o1 && is_alpha_op ob && Fst_then_snd? (rc_a (get_op_a o1) (get_op_a o2)) && Fst_then_snd? (rc_a (get_op_a ob) (get_op_a ol)) then 
-    rc_inter_base_right_a (sel_a l k) (sel_a a k) (sel_a b k) (sel_a c k) (get_op_a o1) (get_op_a o2) (get_op_a ob) (get_op_a ol)
+    rc_inter_base_right_a (sel l ka) (sel a ka) (sel b ka) (sel c ka) (get_op_a o1) (get_op_a o2) (get_op_a ob) (get_op_a ol)
   else if get_key o2 = k && is_beta_op o1 && is_beta_op ob && Fst_then_snd? (rc_b (get_op_b o1) (get_op_b o2)) && Fst_then_snd? (rc_b (get_op_b ob) (get_op_b ol)) then 
-    rc_inter_base_right_b (sel_b l k) (sel_b a k) (sel_b b k) (sel_b c k) (get_op_b o1) (get_op_b o2) (get_op_b ob) (get_op_b ol)
+    rc_inter_base_right_b (sel l kb) (sel a kb) (sel b kb) (sel c kb) (get_op_b o1) (get_op_b o2) (get_op_b ob) (get_op_b ol)
   else rc_inter_base_right_ne l a b c o1 o2 ob ol
 
 val rc_inter_base_left_a (l a b c:concrete_st_a) (o1 o2 ob ol:op_a)
@@ -581,10 +392,11 @@ let rc_inter_base_left (l a b c:concrete_st) (o1 o2 ob ol:op_t)
                     eq (merge l (do a ob) (do b ol)) (do (do c ob) ol)) //***EXTRA***
           (ensures eq (merge (do l ol) (do (do (do a ob) ol) o1) (do (do b ol) o2)) (do (do (do (do c ob) ol) o1) o2)) =
   let k = get_key ob in
+  let ka = Alpha_t k in let kb = Beta_t k in
   if get_key o2 = k && is_alpha_op o1 && is_alpha_op ob && Fst_then_snd? (rc_a (get_op_a o1) (get_op_a o2)) && Fst_then_snd? (rc_a (get_op_a ob) (get_op_a ol)) then 
-    rc_inter_base_left_a (sel_a l k) (sel_a a k) (sel_a b k) (sel_a c k) (get_op_a o1) (get_op_a o2) (get_op_a ob) (get_op_a ol)
+    rc_inter_base_left_a (sel l ka) (sel a ka) (sel b ka) (sel c ka) (get_op_a o1) (get_op_a o2) (get_op_a ob) (get_op_a ol)
   else if get_key o2 = k && is_beta_op o1 && is_beta_op ob && Fst_then_snd? (rc_b (get_op_b o1) (get_op_b o2)) && Fst_then_snd? (rc_b (get_op_b ob) (get_op_b ol)) then 
-    rc_inter_base_left_b (sel_b l k) (sel_b a k) (sel_b b k) (sel_b c k) (get_op_b o1) (get_op_b o2) (get_op_b ob) (get_op_b ol)
+    rc_inter_base_left_b (sel l kb) (sel a kb) (sel b kb) (sel c kb) (get_op_b o1) (get_op_b o2) (get_op_b ob) (get_op_b ol)
   else rc_inter_base_left_ne l a b c o1 o2 ob ol
 
 val rc_inter_right_a (l a b c:concrete_st_a) (o1 o2 ob ol o:op_a)
@@ -628,11 +440,12 @@ let rc_inter_right (l a b c:concrete_st) (o1 o2 ob ol o:op_t)
                     eq (merge (do l ol) (do (do a ol) o1) (do (do (do b ob) ol) o2)) (do (do (do (do c ob) ol) o1) o2))
       (ensures eq (merge (do l ol) (do (do a ol) o1) (do (do (do (do b o) ob) ol) o2)) (do (do (do (do (do c o) ob) ol) o1) o2)) =
   let k = get_key o in
+  let ka = Alpha_t k in let kb = Beta_t k in
   assert (get_key o1 = get_key o2); assert (get_key ob = get_key ol);
   if get_key o2 = k && get_key o2 = get_key ob && is_alpha_op o1 && is_alpha_op o2 && is_alpha_op ob && is_alpha_op ol && is_alpha_op o && Fst_then_snd? (rc_a (get_op_a o1) (get_op_a o2)) && Fst_then_snd? (rc_a (get_op_a ob) (get_op_a ol)) && (Fst_then_snd? (rc_a (get_op_a o) (get_op_a ob)) || Snd_then_fst? (rc_a (get_op_a o) (get_op_a ob)) || Fst_then_snd? (rc_a (get_op_a o) (get_op_a ol))) then 
-    rc_inter_right_a (sel_a l k) (sel_a a k) (sel_a b k) (sel_a c k) (get_op_a o1) (get_op_a o2) (get_op_a ob) (get_op_a ol) (get_op_a o)
+    rc_inter_right_a (sel l ka) (sel a ka) (sel b ka) (sel c ka) (get_op_a o1) (get_op_a o2) (get_op_a ob) (get_op_a ol) (get_op_a o)
   else if get_key o2 = k && get_key o2 = get_key ob && is_beta_op o1 && is_beta_op ob && is_beta_op o && Fst_then_snd? (rc_b (get_op_b o1) (get_op_b o2)) && Fst_then_snd? (rc_b (get_op_b ob) (get_op_b ol)) && (Fst_then_snd? (rc_b (get_op_b o) (get_op_b ob)) || Snd_then_fst? (rc_b (get_op_b o) (get_op_b ob)) || Fst_then_snd? (rc_b (get_op_b o) (get_op_b ol))) then
-    rc_inter_right_b (sel_b l k) (sel_b a k) (sel_b b k) (sel_b c k) (get_op_b o1) (get_op_b o2) (get_op_b ob) (get_op_b ol) (get_op_b o)
+    rc_inter_right_b (sel l kb) (sel a kb) (sel b kb) (sel c kb) (get_op_b o1) (get_op_b o2) (get_op_b ob) (get_op_b ol) (get_op_b o)
   else rc_inter_right_ne l a b c o1 o2 ob ol o
 
 val rc_inter_left_a (l a b c:concrete_st_a) (o1 o2 ob ol o:op_a)
@@ -676,11 +489,12 @@ let rc_inter_left (l a b c:concrete_st) (o1 o2 ob ol o:op_t)
                     eq (merge (do l ol) (do (do (do a ob) ol) o1) (do (do b ol) o2)) (do (do (do (do c ob) ol) o1) o2))
       (ensures eq (merge (do l ol) (do (do (do (do a o) ob) ol) o1) (do (do b ol) o2)) (do (do (do (do (do c o) ob) ol) o1) o2)) =
   let k = get_key o in
+  let ka = Alpha_t k in let kb = Beta_t k in
   assert (get_key o1 = get_key o2); assert (get_key ob = get_key ol);
   if get_key o1 = k && get_key o2 = get_key ob && is_alpha_op o1 && is_alpha_op o2 && is_alpha_op ob && is_alpha_op ol && is_alpha_op o && Fst_then_snd? (rc_a (get_op_a o1) (get_op_a o2)) && Fst_then_snd? (rc_a (get_op_a ob) (get_op_a ol)) && (Fst_then_snd? (rc_a (get_op_a o) (get_op_a ob)) || Snd_then_fst? (rc_a (get_op_a o) (get_op_a ob)) || Fst_then_snd? (rc_a (get_op_a o) (get_op_a ol))) then 
-    rc_inter_left_a (sel_a l k) (sel_a a k) (sel_a b k) (sel_a c k) (get_op_a o1) (get_op_a o2) (get_op_a ob) (get_op_a ol) (get_op_a o)
+    rc_inter_left_a (sel l ka) (sel a ka) (sel b ka) (sel c ka) (get_op_a o1) (get_op_a o2) (get_op_a ob) (get_op_a ol) (get_op_a o)
   else if get_key o2 = k && get_key o2 = get_key ob && is_beta_op o1 && is_beta_op ob && is_beta_op o && Fst_then_snd? (rc_b (get_op_b o1) (get_op_b o2)) && Fst_then_snd? (rc_b (get_op_b ob) (get_op_b ol)) && (Fst_then_snd? (rc_b (get_op_b o) (get_op_b ob)) || Snd_then_fst? (rc_b (get_op_b o) (get_op_b ob)) || Fst_then_snd? (rc_b (get_op_b o) (get_op_b ol))) then
-    rc_inter_left_b (sel_b l k) (sel_b a k) (sel_b b k) (sel_b c k) (get_op_b o1) (get_op_b o2) (get_op_b ob) (get_op_b ol) (get_op_b o)
+    rc_inter_left_b (sel l kb) (sel a kb) (sel b kb) (sel c kb) (get_op_b o1) (get_op_b o2) (get_op_b ob) (get_op_b ol) (get_op_b o)
   else rc_inter_left_ne l a b c o1 o2 ob ol o
 
 //CHECK!!
@@ -725,10 +539,11 @@ let rc_inter_lca (l a b c:concrete_st) (o1 o2 ol oi:op_t)
                     eq (merge (do l ol) (do (do a ol) o1) (do (do b ol) o2)) (do (do (do c ol) o1) o2))
     (ensures eq (merge (do (do l oi) ol) (do (do (do a oi) ol) o1) (do (do (do b oi) ol) o2)) (do (do (do (do c oi) ol) o1) o2)) =
   let k = get_key oi in
+  let ka = Alpha_t k in let kb = Beta_t k in
   if get_key o2 = get_key o1 && get_key o1 = k && get_key o1 = get_key ol && is_alpha_op o1 && is_alpha_op ol && is_alpha_op oi then 
-    rc_inter_lca_a (sel_a l k) (sel_a a k) (sel_a b k) (sel_a c k) (get_op_a o1) (get_op_a o2) (get_op_a ol) (get_op_a oi)
+    rc_inter_lca_a (sel l ka) (sel a ka) (sel b ka) (sel c ka) (get_op_a o1) (get_op_a o2) (get_op_a ol) (get_op_a oi)
   else if get_key o2 = get_key o1 && get_key o1 = k && get_key o1 = get_key ol && is_beta_op o1 && is_beta_op ol && is_beta_op oi then 
-    rc_inter_lca_b (sel_b l k) (sel_b a k) (sel_b b k) (sel_b c k) (get_op_b o1) (get_op_b o2) (get_op_b ol) (get_op_b oi)
+    rc_inter_lca_b (sel l kb) (sel a kb) (sel b kb) (sel c kb) (get_op_b o1) (get_op_b o2) (get_op_b ol) (get_op_b oi)
   else rc_inter_lca_ne l a b c o1 o2 ol oi
 
 (*One op*)
@@ -754,10 +569,11 @@ let one_op_ind_right (l a b:concrete_st) (o2 o2':op_t)
    : Lemma (requires distinct_ops o2 o2' /\ eq (merge l a (do b o2)) (do (merge l a b) o2))
            (ensures eq (merge l a (do (do b o2') o2)) (do (merge l a (do b o2')) o2)) =
   let k = get_key o2' in
+  let ka = Alpha_t k in let kb = Beta_t k in
   if get_key o2 = k && is_alpha_op o2 && is_alpha_op o2' then
-    one_op_ind_right_a (sel_a l k) (sel_a a k) (sel_a b k) (get_op_a o2) (get_op_a o2')
+    one_op_ind_right_a (sel l ka) (sel a ka) (sel b ka) (get_op_a o2) (get_op_a o2')
   else if get_key o2 = k && is_beta_op o2 && is_beta_op o2' then
-    one_op_ind_right_b (sel_b l k) (sel_b a k) (sel_b b k) (get_op_b o2) (get_op_b o2')
+    one_op_ind_right_b (sel l kb) (sel a kb) (sel b kb) (get_op_b o2) (get_op_b o2')
   else one_op_ind_right_ne l a b o2 o2'
 
 val one_op_ind_left_a (l a b:concrete_st_a) (o1 o1':op_a) 
@@ -782,10 +598,11 @@ let one_op_ind_left (l a b:concrete_st) (o1 o1':op_t)
                      eq (merge l (do a o1) b) (do (merge l a b) o1))
            (ensures eq (merge l (do (do a o1') o1) b) (do (merge l (do a o1') b) o1)) =
   let k = get_key o1' in
+  let ka = Alpha_t k in let kb = Beta_t k in
   if get_key o1 = k && is_alpha_op o1 && is_alpha_op o1' then
-    one_op_ind_left_a (sel_a l k) (sel_a a k) (sel_a b k) (get_op_a o1) (get_op_a o1')
+    one_op_ind_left_a (sel l ka) (sel a ka) (sel b ka) (get_op_a o1) (get_op_a o1')
   else if get_key o1 = k && is_beta_op o1 && is_beta_op o1' then
-    one_op_ind_left_b (sel_b l k) (sel_b a k) (sel_b b k) (get_op_b o1) (get_op_b o1')
+    one_op_ind_left_b (sel l kb) (sel a kb) (sel b kb) (get_op_b o1) (get_op_b o1')
   else one_op_ind_left_ne l a b o1 o1'
 
 val one_op_ind_lca_a (l:concrete_st_a) (o2 o:op_a) 
@@ -810,10 +627,11 @@ let one_op_ind_lca (l:concrete_st) (o2 o:op_t)
                      eq (merge l l (do l o2)) (do l o2))
           (ensures eq (merge (do l o) (do l o) (do (do l o) o2)) (do (do l o) o2)) =
   let k = get_key o in
+  let ka = Alpha_t k in let kb = Beta_t k in
   if get_key o2 = k && is_alpha_op o2 && is_alpha_op o then
-    one_op_ind_lca_a (sel_a l k) (get_op_a o2) (get_op_a o)
+    one_op_ind_lca_a (sel l ka) (get_op_a o2) (get_op_a o)
   else if get_key o2 = k && is_beta_op o2 && is_beta_op o then
-    one_op_ind_lca_b (sel_b l k) (get_op_b o2) (get_op_b o)
+    one_op_ind_lca_b (sel l kb) (get_op_b o2) (get_op_b o)
   else one_op_ind_lca_ne l o2 o
 
 val one_op_base_a (o2:op_a)
@@ -822,7 +640,7 @@ val one_op_base_a (o2:op_a)
 val one_op_base_b (o2:op_b)
   : Lemma (ensures eq_b (merge_b init_st_b init_st_b (do_b init_st_b o2)) (do_b init_st_b o2))
 
-let one_op_base (o2:op_t) (t:key_t)
+let one_op_base (o2:op_t) (t:kt)
   : Lemma (ensures eq (merge (init_st t) (init_st t) (do (init_st t) o2)) (do (init_st t) o2)) =
   if is_alpha_op o2 then one_op_base_a (get_op_a o2)
   else one_op_base_b (get_op_b o2)
@@ -862,10 +680,11 @@ let one_op_inter_base_right (l a b c:concrete_st) (o2 ob ol:op_t)
                     eq (merge l (do a ol) (do b ob)) (do (do c ob) ol)) //***EXTRA***
           (ensures eq (merge (do l ol) (do a ol) (do (do (do b ob) ol) o2)) (do (do (do c ob) ol) o2)) =
   let k = get_key ob in
+  let ka = Alpha_t k in let kb = Beta_t k in
   if get_key ol = k && get_key o2 = k && is_alpha_op ob && is_alpha_op ol && is_alpha_op o2 && Fst_then_snd? (rc_a (get_op_a ob) (get_op_a ol)) then
-    one_op_inter_base_right_a (sel_a l k) (sel_a a k) (sel_a b k) (sel_a c k) (get_op_a o2) (get_op_a ob) (get_op_a ol)
+    one_op_inter_base_right_a (sel l ka) (sel a ka) (sel b ka) (sel c ka) (get_op_a o2) (get_op_a ob) (get_op_a ol)
   else if get_key ol = k && get_key o2 = k && is_beta_op ob && is_beta_op ol && is_beta_op o2 && Fst_then_snd? (rc_b (get_op_b ob) (get_op_b ol)) then
-    one_op_inter_base_right_b (sel_b l k) (sel_b a k) (sel_b b k) (sel_b c k) (get_op_b o2) (get_op_b ob) (get_op_b ol)
+    one_op_inter_base_right_b (sel l kb) (sel a kb) (sel b kb) (sel c kb) (get_op_b o2) (get_op_b ob) (get_op_b ol)
   else one_op_inter_base_right_ne l a b c o2 ob ol
 
 val one_op_inter_base_left_a (l a b c:concrete_st_a) (o2 ob ol:op_a) 
@@ -911,10 +730,11 @@ let one_op_inter_base_left (l a b c:concrete_st) (o2 ob ol:op_t)
                     eq (merge l (do a ob) (do b ol)) (do (do c ob) ol)) //***EXTRA***
           (ensures eq (merge (do l ol) (do (do a ob) ol) (do (do b ol) o2)) (do (do (do c ob) ol) o2)) = 
   let k = get_key ob in
+  let ka = Alpha_t k in let kb = Beta_t k in
   if get_key ol = k && get_key o2 = k && is_alpha_op ob && is_alpha_op ol && is_alpha_op o2 && Fst_then_snd? (rc_a (get_op_a ob) (get_op_a ol)) then
-    one_op_inter_base_left_a (sel_a l k) (sel_a a k) (sel_a b k) (sel_a c k) (get_op_a o2) (get_op_a ob) (get_op_a ol)
+    one_op_inter_base_left_a (sel l ka) (sel a ka) (sel b ka) (sel c ka) (get_op_a o2) (get_op_a ob) (get_op_a ol)
   else if get_key ol = k && get_key o2 = k && is_beta_op ob && is_beta_op ol && is_beta_op o2 && Fst_then_snd? (rc_b (get_op_b ob) (get_op_b ol)) then
-    one_op_inter_base_left_b (sel_b l k) (sel_b a k) (sel_b b k) (sel_b c k) (get_op_b o2) (get_op_b ob) (get_op_b ol)
+    one_op_inter_base_left_b (sel l kb) (sel a kb) (sel b kb) (sel c kb) (get_op_b o2) (get_op_b ob) (get_op_b ol)
   else one_op_inter_base_left_ne l a b c o2 ob ol
 
 val one_op_inter_right_a (l a b c:concrete_st_a) (o2 ob ol o:op_a) 
@@ -937,10 +757,11 @@ val one_op_inter_right_ne (l a b c:concrete_st) (o2 ob ol o:op_t)
   : Lemma (requires Fst_then_snd? (rc ob ol) /\
                     distinct_ops o ob /\ distinct_ops o ol /\ distinct_ops o ol /\ distinct_ops ob ol /\ distinct_ops ob o2 /\ distinct_ops o2 ol /\
                     get_rid o <> get_rid ol (*o,ol must be concurrent*) /\
-                    ~ (get_key o = get_key ob && get_key o = get_key ol /\ get_key o = get_key o2 /\
-                       (is_alpha_op ob && is_alpha_op ol && is_alpha_op o2 && is_alpha_op o && Fst_then_snd? (rc_a (get_op_a ob) (get_op_a ol))) /\
-                       (is_beta_op ob && is_beta_op ol && is_beta_op o2 && is_alpha_op o && Fst_then_snd? (rc_b (get_op_b ob) (get_op_b ol)))) /\
-                    (~ (Either? (rc o ob)) \/ Fst_then_snd? (rc o ol)) /\
+                    ~ (get_key o2 = get_key o /\ get_key o2 = get_key ob /\
+                       (is_alpha_op o2 /\ is_alpha_op ob /\ is_alpha_op ol /\ is_alpha_op o /\ Fst_then_snd? (rc_a (get_op_a ob) (get_op_a ol))) /\
+                       (is_beta_op o2 /\ is_beta_op ob /\ is_beta_op ol /\ is_beta_op o /\ Fst_then_snd? (rc_b (get_op_b ob) (get_op_b ol))) /\
+                       (~ (Either? (rc_a (get_op_a o) (get_op_a ob))) \/ Fst_then_snd? (rc_a (get_op_a o) (get_op_a ol))) /\
+                       (~ (Either? (rc_b (get_op_b o) (get_op_b ob))) \/ Fst_then_snd? (rc_b (get_op_b o) (get_op_b ol)))) /\
                     eq (merge (do l ol) (do a ol) (do (do (do b ob) ol) o2)) (do (do (do c ob) ol) o2))
           (ensures eq (merge (do l ol) (do a ol) (do (do (do (do b o) ob) ol) o2)) (do (do (do (do c o) ob) ol) o2))
           
@@ -952,10 +773,11 @@ let one_op_inter_right (l a b c:concrete_st) (o2 ob ol o:op_t)
                     eq (merge (do l ol) (do a ol) (do (do (do b ob) ol) o2)) (do (do (do c ob) ol) o2))
           (ensures eq (merge (do l ol) (do a ol) (do (do (do (do b o) ob) ol) o2)) (do (do (do (do c o) ob) ol) o2)) =
   let k = get_key o in
+  let ka = Alpha_t k in let kb = Beta_t k in
   if get_key ob = k && get_key ol = k && get_key o2 = k && is_alpha_op o && is_alpha_op ob && is_alpha_op ol && is_alpha_op o2 && Fst_then_snd? (rc_a (get_op_a ob) (get_op_a ol)) then
-    one_op_inter_right_a (sel_a l k) (sel_a a k) (sel_a b k) (sel_a c k) (get_op_a o2) (get_op_a ob) (get_op_a ol) (get_op_a o)
-  else if get_key ol = k && get_key o2 = k && is_beta_op ob && is_beta_op ol && is_beta_op o2 && Fst_then_snd? (rc_b (get_op_b ob) (get_op_b ol)) then
-    one_op_inter_right_b (sel_b l k) (sel_b a k) (sel_b b k) (sel_b c k) (get_op_b o2) (get_op_b ob) (get_op_b ol) (get_op_b o)
+    one_op_inter_right_a (sel l ka) (sel a ka) (sel b ka) (sel c ka) (get_op_a o2) (get_op_a ob) (get_op_a ol) (get_op_a o)
+  else if get_key ob = k && get_key ol = k && get_key o2 = k && is_beta_op o && is_beta_op ob && is_beta_op ol && is_beta_op o2 && Fst_then_snd? (rc_b (get_op_b ob) (get_op_b ol)) then
+    one_op_inter_right_b (sel l kb) (sel a kb) (sel b kb) (sel c kb) (get_op_b o2) (get_op_b ob) (get_op_b ol) (get_op_b o)
   else one_op_inter_right_ne l a b c o2 ob ol o
 
 val one_op_inter_left_a (l a b c:concrete_st_a) (o2 ob ol o:op_a) 
@@ -977,11 +799,12 @@ val one_op_inter_left_b (l a b c:concrete_st_b) (o2 ob ol o:op_b)
 val one_op_inter_left_ne (l a b c:concrete_st) (o2 ob ol o:op_t) 
   : Lemma (requires Fst_then_snd? (rc ob ol) /\
                     distinct_ops o ob /\ distinct_ops o ol /\ distinct_ops o ol /\ distinct_ops ob ol /\ distinct_ops ob o2 /\ distinct_ops o2 ol /\
+                    ~ (get_key o2 = get_key o /\ get_key o2 = get_key ob /\
+                       (is_alpha_op o2 /\ is_alpha_op ob /\ is_alpha_op ol /\ is_alpha_op o /\ Fst_then_snd? (rc_a (get_op_a ob) (get_op_a ol))) /\
+                       (is_beta_op o2 /\ is_beta_op ob /\ is_beta_op ol /\ is_beta_op o /\ Fst_then_snd? (rc_b (get_op_b ob) (get_op_b ol))) /\
+                       (~ (Either? (rc_a (get_op_a o) (get_op_a ob))) \/ Fst_then_snd? (rc_a (get_op_a o) (get_op_a ol))) /\
+                       (~ (Either? (rc_b (get_op_b o) (get_op_b ob))) \/ Fst_then_snd? (rc_b (get_op_b o) (get_op_b ol)))) /\
                     get_rid o <> get_rid ol (*o,ol must be concurrent*) /\
-                    ~ (get_key o = get_key ob && get_key o = get_key ol /\ get_key o = get_key o2 /\
-                       (is_alpha_op ob && is_alpha_op ol && is_alpha_op o2 && is_alpha_op o && Fst_then_snd? (rc_a (get_op_a ob) (get_op_a ol))) /\
-                       (is_beta_op ob && is_beta_op ol && is_beta_op o2 && is_alpha_op o && Fst_then_snd? (rc_b (get_op_b ob) (get_op_b ol)))) /\
-                    (~ (Either? (rc o ob)) \/ Fst_then_snd? (rc o ol)) /\
                     eq (merge (do l ol) (do (do a ob) ol) (do (do b ol) o2)) (do (do (do c ob) ol) o2))
           (ensures eq (merge (do l ol) (do (do (do a o) ob) ol) (do (do b ol) o2)) (do (do (do (do c o) ob) ol) o2))
           
@@ -993,10 +816,11 @@ let one_op_inter_left (l a b c:concrete_st) (o2 ob ol o:op_t)
                     eq (merge (do l ol) (do (do a ob) ol) (do (do b ol) o2)) (do (do (do c ob) ol) o2))
           (ensures eq (merge (do l ol) (do (do (do a o) ob) ol) (do (do b ol) o2)) (do (do (do (do c o) ob) ol) o2)) =
   let k = get_key o in
+  let ka = Alpha_t k in let kb = Beta_t k in
   if get_key ob = k && get_key ol = k && get_key o2 = k && is_alpha_op o && is_alpha_op ob && is_alpha_op ol && is_alpha_op o2 && Fst_then_snd? (rc_a (get_op_a ob) (get_op_a ol)) then
-    one_op_inter_left_a (sel_a l k) (sel_a a k) (sel_a b k) (sel_a c k) (get_op_a o2) (get_op_a ob) (get_op_a ol) (get_op_a o)
-  else if get_key ol = k && get_key o2 = k && is_beta_op ob && is_beta_op ol && is_beta_op o2 && Fst_then_snd? (rc_b (get_op_b ob) (get_op_b ol)) then
-    one_op_inter_left_b (sel_b l k) (sel_b a k) (sel_b b k) (sel_b c k) (get_op_b o2) (get_op_b ob) (get_op_b ol) (get_op_b o)
+    one_op_inter_left_a (sel l ka) (sel a ka) (sel b ka) (sel c ka) (get_op_a o2) (get_op_a ob) (get_op_a ol) (get_op_a o)
+  else if get_key ob = k && get_key ol = k && get_key o2 = k && is_beta_op o && is_beta_op ob && is_beta_op ol && is_beta_op o2 && Fst_then_snd? (rc_b (get_op_b ob) (get_op_b ol)) then
+    one_op_inter_left_b (sel l kb) (sel a kb) (sel b kb) (sel c kb) (get_op_b o2) (get_op_b ob) (get_op_b ol) (get_op_b o)
   else one_op_inter_left_ne l a b c o2 ob ol o
 
 val one_op_inter_lca_a (l a b c:concrete_st_a) (o2 ol oi o:op_a)
@@ -1030,10 +854,11 @@ let one_op_inter_lca (l a b c:concrete_st) (o2 ol oi o:op_t)
                     eq (merge (do l ol) (do a ol) (do (do b ol) o2)) (do (do c ol) o2))
           (ensures eq (merge (do (do l oi) ol) (do (do a oi) ol) (do (do (do b oi) ol) o2)) (do (do (do c oi) ol) o2)) =
   let k = get_key oi in
+  let ka = Alpha_t k in let kb = Beta_t k in
   if get_key ol = k && get_key o2 = k && is_alpha_op oi && is_alpha_op ol && is_alpha_op o2 && is_alpha_op o && Fst_then_snd? (rc_a (get_op_a o) (get_op_a ol)) && Fst_then_snd? (rc_a (get_op_a o) (get_op_a oi)) then
-    one_op_inter_lca_a (sel_a l k) (sel_a a k) (sel_a b k) (sel_a c k) (get_op_a o2) (get_op_a ol) (get_op_a oi) (get_op_a o)
+    one_op_inter_lca_a (sel l ka) (sel a ka) (sel b ka) (sel c ka) (get_op_a o2) (get_op_a ol) (get_op_a oi) (get_op_a o)
   else if get_key ol = k && get_key o2 = k && is_beta_op oi && is_beta_op ol && is_beta_op o2 && is_beta_op o && Fst_then_snd? (rc_b (get_op_b o) (get_op_b ol)) && Fst_then_snd? (rc_b (get_op_b o) (get_op_b oi)) then
-    one_op_inter_lca_b (sel_b l k) (sel_b a k) (sel_b b k) (sel_b c k) (get_op_b o2) (get_op_b ol) (get_op_b oi) (get_op_b o)
+    one_op_inter_lca_b (sel l kb) (sel a kb) (sel b kb) (sel c kb) (get_op_b o2) (get_op_b ol) (get_op_b oi) (get_op_b o)
   else one_op_inter_lca_ne l a b c o2 ol oi o
 
 (*Zero op *)
@@ -1072,10 +897,11 @@ let zero_op_inter_base_right (l a b c:concrete_st) (ob ol:op_t)
                     eq (merge l (do a ol) (do b ob)) (do (do c ob) ol)) //***EXTRA***
           (ensures eq (merge (do l ol) (do a ol) (do (do b ob) ol)) (do (do c ob) ol)) =
   let k = get_key ob in
+  let ka = Alpha_t k in let kb = Beta_t k in
   if get_key ol = k && is_alpha_op ob && is_alpha_op ol && Fst_then_snd? (rc_a (get_op_a ob) (get_op_a ol)) then
-    zero_op_inter_base_right_a (sel_a l k) (sel_a a k) (sel_a b k) (sel_a c k) (get_op_a ob) (get_op_a ol)
+    zero_op_inter_base_right_a (sel l ka) (sel a ka) (sel b ka) (sel c ka) (get_op_a ob) (get_op_a ol)
   else if get_key ol = k && is_beta_op ob && is_beta_op ol && Fst_then_snd? (rc_b (get_op_b ob) (get_op_b ol)) then
-    zero_op_inter_base_right_b (sel_b l k) (sel_b a k) (sel_b b k) (sel_b c k) (get_op_b ob) (get_op_b ol)
+    zero_op_inter_base_right_b (sel l kb) (sel a kb) (sel b kb) (sel c kb) (get_op_b ob) (get_op_b ol)
   else zero_op_inter_base_right_ne l a b c ob ol
 
 val zero_op_inter_base_left_a (l a b c:concrete_st_a) (ob ol:op_a) 
@@ -1109,10 +935,11 @@ let zero_op_inter_base_left (l a b c:concrete_st) (ob ol:op_t)
                     eq (merge l (do a ob) (do b ol)) (do (do c ob) ol)) //***EXTRA***
           (ensures eq (merge (do l ol) (do (do a ob) ol) (do b ol)) (do (do c ob) ol)) =
   let k = get_key ob in
+  let ka = Alpha_t k in let kb = Beta_t k in
   if get_key ol = k && is_alpha_op ob && is_alpha_op ol && Fst_then_snd? (rc_a (get_op_a ob) (get_op_a ol)) then
-    zero_op_inter_base_left_a (sel_a l k) (sel_a a k) (sel_a b k) (sel_a c k) (get_op_a ob) (get_op_a ol)
+    zero_op_inter_base_left_a (sel l ka) (sel a ka) (sel b ka) (sel c ka) (get_op_a ob) (get_op_a ol)
   else if get_key ol = k && is_beta_op ob && is_beta_op ol && Fst_then_snd? (rc_b (get_op_b ob) (get_op_b ol)) then
-    zero_op_inter_base_left_b (sel_b l k) (sel_b a k) (sel_b b k) (sel_b c k) (get_op_b ob) (get_op_b ol)
+    zero_op_inter_base_left_b (sel l kb) (sel a kb) (sel b kb) (sel c kb) (get_op_b ob) (get_op_b ol)
   else zero_op_inter_base_left_ne l a b c ob ol
 
 val zero_op_inter_right_a (l a b c:concrete_st_a) (ob ol o:op_a) 
@@ -1150,10 +977,11 @@ let zero_op_inter_right (l a b c:concrete_st) (ob ol o:op_t)
                     eq (merge (do l ol) (do a ol) (do (do b ob) ol)) (do (do c ob) ol))
           (ensures eq (merge (do l ol) (do a ol) (do (do (do b o) ob) ol)) (do (do (do c o) ob) ol)) =
   let k = get_key o in
+  let ka = Alpha_t k in let kb = Beta_t k in
   if get_key ob = k && get_key ol = k && is_alpha_op o && is_alpha_op ob && is_alpha_op ol && Fst_then_snd? (rc_a (get_op_a ob) (get_op_a ol)) then
-    zero_op_inter_right_a (sel_a l k) (sel_a a k) (sel_a b k) (sel_a c k) (get_op_a ob) (get_op_a ol) (get_op_a o)
+    zero_op_inter_right_a (sel l ka) (sel a ka) (sel b ka) (sel c ka) (get_op_a ob) (get_op_a ol) (get_op_a o)
   else if get_key ol = k && is_beta_op ob && is_beta_op ol && Fst_then_snd? (rc_b (get_op_b ob) (get_op_b ol)) then
-    zero_op_inter_right_b (sel_b l k) (sel_b a k) (sel_b b k) (sel_b c k) (get_op_b ob) (get_op_b ol) (get_op_b o)
+    zero_op_inter_right_b (sel l kb) (sel a kb) (sel b kb) (sel c kb) (get_op_b ob) (get_op_b ol) (get_op_b o)
   else zero_op_inter_right_ne l a b c ob ol o
 
 val zero_op_inter_left_a (l a b c:concrete_st_a) (ob ol o:op_a) 
@@ -1191,10 +1019,11 @@ let zero_op_inter_left (l a b c:concrete_st) (ob ol o:op_t)
                     eq (merge (do l ol) (do (do a ob) ol) (do b ol)) (do (do c ob) ol))
           (ensures eq (merge (do l ol) (do (do (do a o) ob) ol) (do b ol)) (do (do (do c o) ob) ol)) =
   let k = get_key o in
+  let ka = Alpha_t k in let kb = Beta_t k in
   if get_key ob = k && get_key ol = k && is_alpha_op o && is_alpha_op ob && is_alpha_op ol && Fst_then_snd? (rc_a (get_op_a ob) (get_op_a ol)) then
-    zero_op_inter_left_a (sel_a l k) (sel_a a k) (sel_a b k) (sel_a c k) (get_op_a ob) (get_op_a ol) (get_op_a o)
+    zero_op_inter_left_a (sel l ka) (sel a ka) (sel b ka) (sel c ka) (get_op_a ob) (get_op_a ol) (get_op_a o)
   else if get_key ol = k && is_beta_op ob && is_beta_op ol && Fst_then_snd? (rc_b (get_op_b ob) (get_op_b ol)) then
-    zero_op_inter_left_b (sel_b l k) (sel_b a k) (sel_b b k) (sel_b c k) (get_op_b ob) (get_op_b ol) (get_op_b o)
+    zero_op_inter_left_b (sel l kb) (sel a kb) (sel b kb) (sel c kb) (get_op_b ob) (get_op_b ol) (get_op_b o)
   else zero_op_inter_left_ne l a b c ob ol o
 
 val zero_op_inter_lca_v1_a (l a b c:concrete_st_a) (ol:op_a)
@@ -1209,8 +1038,9 @@ let zero_op_inter_lca_v1 (l a b c:concrete_st) (ol:op_t)
   : Lemma (requires (exists o'. Fst_then_snd? (rc o' ol)) /\ eq (merge l a b) c)
           (ensures eq (merge (do l ol) (do a ol) (do b ol)) (do c ol)) =
   let k = get_key ol in
-  if is_alpha_op ol then zero_op_inter_lca_v1_a (sel_a l k) (sel_a a k) (sel_a b k) (sel_a c k) (get_op_a ol)
-  else zero_op_inter_lca_v1_b (sel_b l k) (sel_b a k) (sel_b b k) (sel_b c k) (get_op_b ol)
+  let ka = Alpha_t k in let kb = Beta_t k in
+  if is_alpha_op ol then zero_op_inter_lca_v1_a (sel l ka) (sel a ka) (sel b ka) (sel c ka) (get_op_a ol)
+  else zero_op_inter_lca_v1_b (sel l kb) (sel a kb) (sel b kb) (sel c kb) (get_op_b ol)
 
 val zero_op_inter_lca_v2_a (l a b c:concrete_st_a) (ol oi:op_a)
   : Lemma (requires (exists o'. Fst_then_snd? (rc_a o' ol)) /\
@@ -1243,8 +1073,9 @@ let zero_op_inter_lca_v2 (l a b c:concrete_st) (ol oi:op_t)
                     eq (merge (do l ol) (do a ol) (do b ol)) (do c ol))
           (ensures eq (merge (do (do l oi) ol) (do (do a oi) ol) (do (do b oi) ol)) (do (do c oi) ol)) =
   let k = get_key oi in
-  if get_key ol = k && is_alpha_op ol && is_alpha_op oi then zero_op_inter_lca_v2_a (sel_a l k) (sel_a a k) (sel_a b k) (sel_a c k) (get_op_a ol) (get_op_a oi)
-  else if get_key ol = k && is_beta_op ol && is_beta_op oi then zero_op_inter_lca_v2_b (sel_b l k) (sel_b a k) (sel_b b k) (sel_b c k) (get_op_b ol) (get_op_b oi)
+  let ka = Alpha_t k in let kb = Beta_t k in
+  if get_key ol = k && is_alpha_op ol && is_alpha_op oi then zero_op_inter_lca_v2_a (sel l ka) (sel a ka) (sel b ka) (sel c ka) (get_op_a ol) (get_op_a oi)
+  else if get_key ol = k && is_beta_op ol && is_beta_op oi then zero_op_inter_lca_v2_b (sel l kb) (sel a kb) (sel b kb) (sel c kb) (get_op_b ol) (get_op_b oi)
   else zero_op_inter_lca_v2_ne l a b c ol oi
 
 (* 2 op Comm  *)
@@ -1289,10 +1120,11 @@ let comm_ind_right (l a b:concrete_st) (o1 o2 o2':op_t)
                     ~ (exists o3 b'. eq (do b o2) (do b' o3) /\ distinct_ops o1 o3 /\ Fst_then_snd? (rc o1 o3)))                    
           (ensures eq (merge l (do a o1) (do (do b o2') o2)) (do (do (merge l a (do b o2')) o2) o1)) =
   let k = get_key o2' in
+  let ka = Alpha_t k in let kb = Beta_t k in
   if get_key o2 = k && get_key o1 = k && is_alpha_op o1 && is_alpha_op o2' && is_alpha_op o2 && Either? (rc_a (get_op_a o1) (get_op_a o2)) then
-    comm_ind_right_a (sel_a l k) (sel_a a k) (sel_a b k) (get_op_a o1) (get_op_a o2) (get_op_a o2')
+    comm_ind_right_a (sel l ka) (sel a ka) (sel b ka) (get_op_a o1) (get_op_a o2) (get_op_a o2')
   else if get_key o2 = k && get_key o1 = k && is_beta_op o1 && is_beta_op o2' && is_beta_op o2 && Either? (rc_b (get_op_b o1) (get_op_b o2)) then 
-    comm_ind_right_b (sel_b l k) (sel_b a k) (sel_b b k) (get_op_b o1) (get_op_b o2) (get_op_b o2')
+    comm_ind_right_b (sel l kb) (sel a kb) (sel b kb) (get_op_b o1) (get_op_b o2) (get_op_b o2')
   else comm_ind_right_ne l a b o1 o2 o2'
 
 val comm_ind_left_a (l a b:concrete_st_a) (o1 o2 o1':op_a)
@@ -1334,10 +1166,11 @@ let comm_ind_left (l a b:concrete_st) (o1 o2 o1':op_t)
                     ~ (exists o3 b'. eq (do b o2) (do b' o3) /\ distinct_ops o1 o3 /\ Fst_then_snd? (rc o1 o3)))                    
           (ensures eq (merge l (do (do a o1') o1) (do b o2)) (do (do (merge l (do a o1') b) o2) o1)) =
   let k = get_key o1' in
+  let ka = Alpha_t k in let kb = Beta_t k in
   if get_key o2 = k && get_key o1 = k && is_alpha_op o1 && is_alpha_op o1' && is_alpha_op o2 && Either? (rc_a (get_op_a o1) (get_op_a o2)) then
-    comm_ind_left_a (sel_a l k) (sel_a a k) (sel_a b k) (get_op_a o1) (get_op_a o2) (get_op_a o1')
+    comm_ind_left_a (sel l ka) (sel a ka) (sel b ka) (get_op_a o1) (get_op_a o2) (get_op_a o1')
   else if get_key o2 = k && get_key o1 = k && is_beta_op o1 && is_beta_op o1' && is_beta_op o2 && Either? (rc_b (get_op_b o1) (get_op_b o2)) then 
-    comm_ind_left_b (sel_b l k) (sel_b a k) (sel_b b k) (get_op_b o1) (get_op_b o2) (get_op_b o1')
+    comm_ind_left_b (sel l kb) (sel a kb) (sel b kb) (get_op_b o1) (get_op_b o2) (get_op_b o1')
   else comm_ind_left_ne l a b o1 o2 o1'
 
 val comm_ind_lca_a (l:concrete_st_a) (ol o1 o2:op_a)
@@ -1364,13 +1197,14 @@ let comm_ind_lca (l:concrete_st) (ol o1 o2:op_t)
                     eq (merge l (do l o1) (do l o2)) (do (do l o2) o1))
           (ensures eq (merge (do l ol) (do (do l ol) o1) (do (do l ol) o2)) (do (do (do l ol) o2) o1)) =
   let k = get_key ol in
+  let ka = Alpha_t k in let kb = Beta_t k in
   if get_key ol = get_key o1 && get_key ol = get_key o2 && is_alpha_op ol && is_alpha_op o1 && is_alpha_op o2 then
-    comm_ind_lca_a (sel_a l k) (get_op_a ol) (get_op_a o1) (get_op_a o2)
+    comm_ind_lca_a (sel l ka) (get_op_a ol) (get_op_a o1) (get_op_a o2)
   else if get_key ol = get_key o1 && get_key ol = get_key o2 && is_beta_op ol && is_beta_op o1 && is_beta_op o2 then
-    comm_ind_lca_b (sel_b l k) (get_op_b ol) (get_op_b o1) (get_op_b o2)
+    comm_ind_lca_b (sel l kb) (get_op_b ol) (get_op_b o1) (get_op_b o2)
   else comm_ind_lca_ne l ol o1 o2
 
-val comm_base (o1 o2:op_t) (t:key_t)
+val comm_base (o1 o2:op_t) (t:kt)
   : Lemma (requires Either? (rc o1 o2) /\ distinct_ops o1 o2)
           (ensures eq (merge (init_st t) (do (init_st t) o1) (do (init_st t) o2)) (do (do (init_st t) o1) o2))
 
@@ -1396,8 +1230,8 @@ val comm_inter_base_right_ne (l a b c:concrete_st) (o1 o2 ob ol:op_t)
   : Lemma (requires Either? (rc o1 o2) /\ Fst_then_snd? (rc ob ol) /\ 
                     distinct_ops o1 o2 /\ distinct_ops o1 ob /\ distinct_ops o1 ol /\ distinct_ops o2 ob /\ distinct_ops o2 ol /\ distinct_ops ob ol /\
                     ~ (get_key ol = get_key ob && get_key o1 = get_key ob && get_key o2 = get_key ob /\
-                       (is_alpha_op o1 /\ is_alpha_op o2 /\ is_alpha_op ob /\ is_alpha_op ol) /\
-                       (is_beta_op o1 /\ is_beta_op o2 /\ is_beta_op ob /\ is_beta_op ol)) /\
+                       (is_alpha_op o1 /\ is_alpha_op o2 /\ is_alpha_op ob /\ is_alpha_op ol /\ Either? (rc_a (get_op_a o1) (get_op_a o2)) /\ Fst_then_snd? (rc_a (get_op_a ob) (get_op_a ol)) /\ Fst_then_snd? (rc_a (get_op_a ob) (get_op_a ol))) /\
+                       (is_beta_op o1 /\ is_beta_op o2 /\ is_beta_op ob /\ is_beta_op ol /\ Either? (rc_b (get_op_b o1) (get_op_b o2)) /\ Fst_then_snd? (rc_b (get_op_b ob) (get_op_b ol)))) /\
                     eq (merge (do l ol) (do (do a ol) o1) (do (do b ol) o2)) (do (do (do c ol) o1) o2) /\ 
                     eq (merge l (do a o1) (do b o2)) (do (do c o1) o2) /\
                     eq (merge l (do a o1) (do (do b ob) o2)) (do (do (merge l a (do b ob)) o1) o2) /\ //comes from comm_ind_right
@@ -1413,10 +1247,11 @@ let comm_inter_base_right (l a b c:concrete_st) (o1 o2 ob ol:op_t)
                     eq (merge (do l ol) (do a ol) (do (do b ob) ol)) (do (do c ob) ol)) //comes from intermediate_base_zero_op
           (ensures eq (merge (do l ol) (do (do a ol) o1) (do (do (do b ob) ol) o2)) (do (do (do (do c ob) ol) o1) o2)) =
   let k = get_key ob in
+  let ka = Alpha_t k in let kb = Beta_t k in
   if get_key ol = k && get_key o1 = k && get_key o2 = k && is_alpha_op o1 && is_alpha_op o2 && is_alpha_op ob && is_alpha_op ol && Either? (rc_a (get_op_a o1) (get_op_a o2)) && Fst_then_snd? (rc_a (get_op_a ob) (get_op_a ol)) then
-    comm_inter_base_right_a (sel_a l k) (sel_a a k) (sel_a b k) (sel_a c k) (get_op_a o1) (get_op_a o2) (get_op_a ob) (get_op_a ol)
+    comm_inter_base_right_a (sel l ka) (sel a ka) (sel b ka) (sel c ka) (get_op_a o1) (get_op_a o2) (get_op_a ob) (get_op_a ol)
   else if get_key ol = k && get_key o1 = k && get_key o2 = k && is_beta_op o1 && is_beta_op o2 && is_beta_op ob && is_beta_op ol && Either? (rc_b (get_op_b o1) (get_op_b o2)) && Fst_then_snd? (rc_b (get_op_b ob) (get_op_b ol)) then
-    comm_inter_base_right_b (sel_b l k) (sel_b a k) (sel_b b k) (sel_b c k) (get_op_b o1) (get_op_b o2) (get_op_b ob) (get_op_b ol)
+    comm_inter_base_right_b (sel l kb) (sel a kb) (sel b kb) (sel c kb) (get_op_b o1) (get_op_b o2) (get_op_b ob) (get_op_b ol)
   else comm_inter_base_right_ne l a b c o1 o2 ob ol
 
 val comm_inter_base_left_a (l a b c:concrete_st_a) (o1 o2 ob ol:op_a) 
@@ -1441,8 +1276,8 @@ val comm_inter_base_left_ne (l a b c:concrete_st) (o1 o2 ob ol:op_t)
   : Lemma (requires Either? (rc o1 o2) /\ Fst_then_snd? (rc ob ol) /\ 
                     distinct_ops o1 o2 /\ distinct_ops o1 ob /\ distinct_ops o1 ol /\ distinct_ops o2 ob /\ distinct_ops o2 ol /\ distinct_ops ob ol /\
                     ~ (get_key ol = get_key ob && get_key o1 = get_key ob && get_key o2 = get_key ob /\
-                       (is_alpha_op o1 /\ is_alpha_op o2 /\ is_alpha_op ob /\ is_alpha_op ol) /\
-                       (is_beta_op o1 /\ is_beta_op o2 /\ is_beta_op ob /\ is_beta_op ol)) /\
+                       (is_alpha_op o1 /\ is_alpha_op o2 /\ is_alpha_op ob /\ is_alpha_op ol /\ Either? (rc_a (get_op_a o1) (get_op_a o2)) /\ Fst_then_snd? (rc_a (get_op_a ob) (get_op_a ol))) /\
+                       (is_beta_op o1 /\ is_beta_op o2 /\ is_beta_op ob /\ is_beta_op ol /\ Either? (rc_b (get_op_b o1) (get_op_b o2)) /\ Fst_then_snd? (rc_b (get_op_b ob) (get_op_b ol)))) /\
                     eq (merge (do l ol) (do (do a ol) o1) (do (do b ol) o2)) (do (do (do c ol) o1) o2) /\ 
                     eq (merge l (do a o1) (do b o2)) (do (do c o1) o2) /\
                     eq (merge l (do a o1) (do (do b ob) o2)) (do (do (merge l a (do b ob)) o1) o2) /\ //comes from comm_ind_left
@@ -1458,10 +1293,11 @@ let comm_inter_base_left (l a b c:concrete_st) (o1 o2 ob ol:op_t)
                     eq (merge (do l ol) (do (do a ob) ol) (do b ol)) (do (do c ob) ol)) //comes from intermediate_base_zero_op
           (ensures eq (merge (do l ol) (do (do (do a ob) ol) o1) (do (do b ol) o2)) (do (do (do (do c ob) ol) o1) o2)) =
   let k = get_key ob in
+  let ka = Alpha_t k in let kb = Beta_t k in
   if get_key ol = k && get_key o1 = k && get_key o2 = k && is_alpha_op o1 && is_alpha_op o2 && is_alpha_op ob && is_alpha_op ol && Either? (rc_a (get_op_a o1) (get_op_a o2)) && Fst_then_snd? (rc_a (get_op_a ob) (get_op_a ol)) then
-    comm_inter_base_left_a (sel_a l k) (sel_a a k) (sel_a b k) (sel_a c k) (get_op_a o1) (get_op_a o2) (get_op_a ob) (get_op_a ol)
+    comm_inter_base_left_a (sel l ka) (sel a ka) (sel b ka) (sel c ka) (get_op_a o1) (get_op_a o2) (get_op_a ob) (get_op_a ol)
   else if get_key ol = k && get_key o1 = k && get_key o2 = k && is_beta_op o1 && is_beta_op o2 && is_beta_op ob && is_beta_op ol && Either? (rc_b (get_op_b o1) (get_op_b o2)) && Fst_then_snd? (rc_b (get_op_b ob) (get_op_b ol)) then
-    comm_inter_base_left_b (sel_b l k) (sel_b a k) (sel_b b k) (sel_b c k) (get_op_b o1) (get_op_b o2) (get_op_b ob) (get_op_b ol)
+    comm_inter_base_left_b (sel l kb) (sel a kb) (sel b kb) (sel c kb) (get_op_b o1) (get_op_b o2) (get_op_b ob) (get_op_b ol)
   else comm_inter_base_left_ne l a b c o1 o2 ob ol
 
 val comm_inter_right_a (l a b c:concrete_st_a) (o1 o2 ob ol o:op_a)
@@ -1505,10 +1341,11 @@ let comm_inter_right (l a b c:concrete_st) (o1 o2 ob ol o:op_t)
                     eq (merge (do l ol) (do (do a ol) o1) (do (do (do b ob) ol) o2)) (do (do (do (do c ob) ol) o1) o2))
           (ensures eq (merge (do l ol) (do (do a ol) o1) (do (do (do (do b o) ob) ol) o2)) (do (do (do (do (do c o) ob) ol) o1) o2)) =
   let k = get_key o in
+  let ka = Alpha_t k in let kb = Beta_t k in
   if get_key o1 = k && get_key o2 = k && get_key ob = k && get_key ol = k && is_alpha_op o1 && is_alpha_op o2 && is_alpha_op ob && is_alpha_op ol && is_alpha_op o && Fst_then_snd? (rc_a (get_op_a o1) (get_op_a o2)) && Fst_then_snd? (rc_a (get_op_a ob) (get_op_a ol)) && (Fst_then_snd? (rc_a (get_op_a o) (get_op_a ob)) || Snd_then_fst? (rc_a (get_op_a o) (get_op_a ob)) || Fst_then_snd? (rc_a (get_op_a o) (get_op_a ol))) then 
-    comm_inter_right_a (sel_a l k) (sel_a a k) (sel_a b k) (sel_a c k) (get_op_a o1) (get_op_a o2) (get_op_a ob) (get_op_a ol) (get_op_a o)
+    comm_inter_right_a (sel l ka) (sel a ka) (sel b ka) (sel c ka) (get_op_a o1) (get_op_a o2) (get_op_a ob) (get_op_a ol) (get_op_a o)
   else if get_key o1 = k && get_key o2 = k && get_key ob = k && get_key ol = k && is_beta_op o1 && is_beta_op o2 && is_beta_op ob && is_beta_op ol && is_beta_op o && Fst_then_snd? (rc_b (get_op_b o1) (get_op_b o2)) && Fst_then_snd? (rc_b (get_op_b ob) (get_op_b ol)) && (Fst_then_snd? (rc_b (get_op_b o) (get_op_b ob)) || Snd_then_fst? (rc_b (get_op_b o) (get_op_b ob)) || Fst_then_snd? (rc_b (get_op_b o) (get_op_b ol))) then
-    comm_inter_right_b (sel_b l k) (sel_b a k) (sel_b b k) (sel_b c k) (get_op_b o1) (get_op_b o2) (get_op_b ob) (get_op_b ol) (get_op_b o)
+    comm_inter_right_b (sel l kb) (sel a kb) (sel b kb) (sel c kb) (get_op_b o1) (get_op_b o2) (get_op_b ob) (get_op_b ol) (get_op_b o)
   else comm_inter_right_ne l a b c o1 o2 ob ol o
 
 val comm_inter_left_a (l a b c:concrete_st_a) (o1 o2 ob ol o:op_a)
@@ -1552,10 +1389,11 @@ let comm_inter_left (l a b c:concrete_st) (o1 o2 ob ol o:op_t)
                     eq (merge (do l ol) (do (do (do a ob) ol) o1) (do (do b ol) o2)) (do (do (do (do c ob) ol) o1) o2))
           (ensures eq (merge (do l ol) (do (do (do (do a o) ob) ol) o1) (do (do b ol) o2)) (do (do (do (do (do c o) ob) ol) o1) o2)) =
   let k = get_key o in
+  let ka = Alpha_t k in let kb = Beta_t k in
   if get_key o1 = k && get_key o2 = k && get_key ob = k && get_key ol = k && is_alpha_op o1 && is_alpha_op o2 && is_alpha_op ob && is_alpha_op ol && is_alpha_op o && Fst_then_snd? (rc_a (get_op_a o1) (get_op_a o2)) && Fst_then_snd? (rc_a (get_op_a ob) (get_op_a ol)) && (Fst_then_snd? (rc_a (get_op_a o) (get_op_a ob)) || Snd_then_fst? (rc_a (get_op_a o) (get_op_a ob)) || Fst_then_snd? (rc_a (get_op_a o) (get_op_a ol))) then 
-    comm_inter_left_a (sel_a l k) (sel_a a k) (sel_a b k) (sel_a c k) (get_op_a o1) (get_op_a o2) (get_op_a ob) (get_op_a ol) (get_op_a o)
+    comm_inter_left_a (sel l ka) (sel a ka) (sel b ka) (sel c ka) (get_op_a o1) (get_op_a o2) (get_op_a ob) (get_op_a ol) (get_op_a o)
   else if get_key o1 = k && get_key o2 = k && get_key ob = k && get_key ol = k && is_beta_op o1 && is_beta_op o2 && is_beta_op ob && is_beta_op ol && is_beta_op o && Fst_then_snd? (rc_b (get_op_b o1) (get_op_b o2)) && Fst_then_snd? (rc_b (get_op_b ob) (get_op_b ol)) && (Fst_then_snd? (rc_b (get_op_b o) (get_op_b ob)) || Snd_then_fst? (rc_b (get_op_b o) (get_op_b ob)) || Fst_then_snd? (rc_b (get_op_b o) (get_op_b ol))) then
-    comm_inter_left_b (sel_b l k) (sel_b a k) (sel_b b k) (sel_b c k) (get_op_b o1) (get_op_b o2) (get_op_b ob) (get_op_b ol) (get_op_b o)
+    comm_inter_left_b (sel l kb) (sel a kb) (sel b kb) (sel c kb) (get_op_b o1) (get_op_b o2) (get_op_b ob) (get_op_b ol) (get_op_b o)
   else comm_inter_left_ne l a b c o1 o2 ob ol o
 
 val comm_inter_lca_a (l a b c:concrete_st_a) (o1 o2 ol:op_a)
@@ -1589,286 +1427,10 @@ let comm_inter_lca (l a b c:concrete_st) (o1 o2 ol:op_t)
                     eq (merge l (do a o1) (do b o2)) (do (do c o1) o2))
           (ensures eq (merge (do l ol) (do (do a ol) o1) (do (do b ol) o2)) (do (do (do c ol) o1) o2)) =
   let k = get_key ol in
+  let ka = Alpha_t k in let kb = Beta_t k in
   if get_key o1 = k && get_key o2 = k && is_alpha_op o1 && is_alpha_op o2 && is_alpha_op ol then
-    comm_inter_lca_a (sel_a l k) (sel_a a k) (sel_a b k) (sel_a c k) (get_op_a o1) (get_op_a o2) (get_op_a ol)
+    comm_inter_lca_a (sel l ka) (sel a ka) (sel b ka) (sel c ka) (get_op_a o1) (get_op_a o2) (get_op_a ol)
   else if get_key o1 = k && get_key o2 = k && is_beta_op o1 && is_beta_op o2 && is_beta_op ol then
-    comm_inter_lca_b (sel_b l k) (sel_b a k) (sel_b b k) (sel_b c k) (get_op_b o1) (get_op_b o2) (get_op_b ol) 
+    comm_inter_lca_b (sel l kb) (sel a kb) (sel b kb) (sel c kb) (get_op_b o1) (get_op_b o2) (get_op_b ol) 
   else comm_inter_lca_ne l a b c o1 o2 ol
 
-
-
-
-
-(*module Polymorphic_gmap
-
-module S = Set_extended
-module M = Map_extended
-open FStar.Seq
-
-#set-options "--query_stats"
-//key type
-type key_t =
-  |Ctr_t
-  |Gset_t
-
-// concrete state of values
-noeq type concrete_st_v = 
-  |Ctr : int -> concrete_st_v
-  |Gset : S.t nat -> concrete_st_v
-
-let eq_key_t (s:M.t (string & key_t) concrete_st_v) =
-  (forall sk. M.contains s sk ==> (let v = M.sel s sk in
-         ((Ctr? v ==> snd sk == Ctr_t) /\ (Gset? v ==> snd sk = Gset_t))))
-
-//concrete state
-let concrete_st = s:M.t (string & key_t) concrete_st_v {eq_key_t s}
-
-let init_st_v (t:key_t) : (s:concrete_st_v{(t == Ctr_t <==> Ctr? s) /\ (t == Gset_t <==> Gset? s)}) =
-  match t with
-  |Ctr_t -> Ctr 0
-  |Gset_t -> Gset S.empty
-
-let init_st (t:key_t) : concrete_st = M.const_on S.empty (init_st_v t)
-
-let sel (s:concrete_st) (t:key_t) k  =
-    if M.contains s (k,t) then M.sel s (k,t) else (init_st_v t)
-
-let eq_ctr (a:concrete_st_v{Ctr? a}) (b:concrete_st_v{Ctr? b}) = 
-  let Ctr c1 = a in 
-  let Ctr c2 = b in
-  c1 = c2
-
-let eq_gset (a:concrete_st_v{Gset? a}) (b:concrete_st_v{Gset? b}) = 
-  let Gset s1 = a in 
-  let Gset s2 = b in
-  S.equal s1 s2
-
-let eq_v (a:concrete_st_v) (b:concrete_st_v) : Type0 = //{(Ctr? a ==> Ctr? b) /\ (Gset? a ==> Gset? b)}) : Type0 =
-  match a,b with
-  |Ctr x,Ctr y -> x = y
-  |Gset x, Gset y -> S.equal x y
-  |_ -> False
-
-// equivalence relation
-let eq (a b:concrete_st) =
-  (forall k t. M.contains a (k,t) = M.contains b (k,t)) /\
-  (forall k t. M.contains a (k,t) ==> eq_v (sel a t k) (sel b t k))
-
-let symmetric (a b:concrete_st) 
-  : Lemma (requires eq a b)
-          (ensures eq b a) = ()
-
-let transitive (a b c:concrete_st)
-  : Lemma (requires eq a b /\ eq b c)
-          (ensures eq a c) = ()
-
-let eq_is_equiv (a b:concrete_st)
-  : Lemma (requires a == b)
-          (ensures eq a b) = ()
-
-type app_op_v : eqtype =
-  |Inc 
-  |Add : nat -> app_op_v
-
-type op_v = pos (*timestamp*) & (nat (*replica ID*) & app_op_v)
-
-//operation type
-type app_op_t:eqtype =
-  |Set : string (* key *) -> app_op_v (* value *) -> app_op_t
-
-let do_v (s:concrete_st_v) (o:op_v) : concrete_st_v =
-  match snd (snd o) with
-  |Inc -> begin match s with
-         |Ctr c -> Ctr (c+1)
-         |_ -> s
-         end
-  |Add v -> begin match s with
-           |Gset s -> Gset (S.add v s)
-           |_ -> s
-           end
-
-type op_t = pos (*timestamp*) & (nat (*replica ID*) & app_op_t)
-
-let get_rid (_,(rid,_)) = rid
-
-let distinct_ops (op1 op2:op_t) = fst op1 =!= fst op2
-
-let get_op_v (o:op_t) : op_v =
-  match o with
-  |(ts,(rid,(Set k op))) -> (ts,(rid,op))
-
-let do_pre (s:concrete_st) (o:op_t) =
-  match o with
-  |(_,(_,Set k opv)) -> begin match opv with
-                       |Inc -> (forall t. M.contains s (k,t) ==> t == Ctr_t)
-                       |Add _ -> (forall t. M.contains s (k,t) ==> t == Gset_t)
-                       end
-
-let do (s:concrete_st) (o:op_t(*{do_pre s o}*)) : concrete_st =
-  match o with
-    |_,(_,Set k Inc) -> (*if M.contains s (k,Ctr_t) then*) M.upd s (k,Ctr_t) (do_v (sel s Ctr_t k) (get_op_v o))
-                       //else M.upd s (k,Ctr_t) (Ctr 1)
-    |_,(_,Set k (Add e)) -> (*if M.contains s (k,Gset_t) then*) M.upd s (k,Gset_t) (do_v (sel s Gset_t k) (get_op_v o))
-                           //else M.upd s (k,Gset_t) (Gset (S.add e S.empty))
-
-type rc_res =
-  |Fst_then_snd //o1 -> o2
-  |Snd_then_fst //o2 -> o1
-  |Either
-  
-//conflict resolution
-let rc (o1:op_t) (o2:op_t(*{distinct_ops o1 o2}*)) : rc_res = Either
-
-let merge_ctr (l a:concrete_st_v) (b:concrete_st_v{Ctr? l /\ Ctr? a /\ Ctr? b}) : concrete_st_v =
-  let Ctr c1 = l in let Ctr c2 = a in let Ctr c3 = b in
-  Ctr (c2 + c3 - c1)
-
-let merge_gset (l a:concrete_st_v) (b:concrete_st_v{Gset? l /\ Gset? a /\ Gset? b}) : concrete_st_v =
-  let Gset s1 = l in let Gset s2 = a in let Gset s3 = b in
-  Gset (S.union s1 (S.union s2 s3))
-
-// concrete merge operation
-let merge (l a b:concrete_st) : concrete_st =
-  let keys = S.union (M.domain l) (S.union (M.domain a) (M.domain b)) in
-  let u = M.const_on keys (0, false) in
-  M.iter_upd (fun (k,t) v -> if Ctr_t? t then merge_ctr (sel l t k) (sel a t k) (sel b t k) 
-                          else merge_gset (sel l t k) (sel a t k) (sel b t k)) u
-
-let commutes_with (o1 o2:op_t) =
-  forall s. eq (do (do s o1) o2) (do (do s o2) o1)
-
-type log = seq op_t
-
-// applying a log of operations to a concrete state
-let rec apply_log (x:concrete_st) (l:log) : Tot concrete_st (decreases length l) =
-  match length l with
-  |0 -> x
-  |_ -> apply_log (do x (head l)) (tail l)  
-
-
-/////////////////////////////////////////////////////////////////////////////
-
-#set-options "--z3rlimit 300 --ifuel 3"
-let rc_non_comm1 (o1 o2:op_t)
-  : Lemma (requires distinct_ops o1 o2)
-          (ensures commutes_with o1 o2 ==> Either? (rc o1 o2)) = ()
-
-let rc_non_comm2 (o1 o2:op_t)
-  : Lemma (requires distinct_ops o1 o2)
-          (ensures Either? (rc o1 o2) ==> commutes_with o1 o2) = ()
-
-let rc_non_comm (o1 o2:op_t)
-  : Lemma (requires distinct_ops o1 o2)
-          (ensures Either? (rc o1 o2) <==> commutes_with o1 o2) = 
-  rc_non_comm1 o1 o2;
-  rc_non_comm2 o1 o2
-
-let no_rc_chain (o1 o2 o3:op_t)
-  : Lemma (requires distinct_ops o1 o2 /\ distinct_ops o2 o3)
-          (ensures ~ (Fst_then_snd? (rc o1 o2) /\ Fst_then_snd? (rc o2 o3))) = ()
-
-let cond_comm_base (s:concrete_st) (o1 o2 o3:op_t) 
-  : Lemma (requires distinct_ops o1 o2 /\ distinct_ops o2 o3 /\ distinct_ops o1 o3 /\
-                    Fst_then_snd? (rc o1 o2) /\ ~ (Either? (rc o2 o3)))
-          (ensures eq (do (do (do s o1) o2) o3) (do (do (do s o2) o1) o3)) = ()
-
-let cond_comm_ind (s:concrete_st) (o1 o2 o3 o:op_t) (l:seq op_t)
-  : Lemma (requires distinct_ops o1 o2 /\ distinct_ops o1 o3 /\ distinct_ops o2 o3 /\ 
-                    Fst_then_snd? (rc o1 o2) /\ ~ (Either? (rc o2 o3)) /\
-                    eq (do (apply_log (do (do s o1) o2) l) o3) (do (apply_log (do (do s o2) o1) l) o3))
-          (ensures eq (do (do (apply_log (do (do s o1) o2) l) o) o3) (do (do (apply_log (do (do s o2) o1) l) o) o3)) = ()
-
-////////////////////////////////////////////////////////////////////////////
-
-let merge_comm (l a b:concrete_st)
-  : Lemma (ensures (eq (merge l a b) (merge l b a))) = ()
-                       
-let merge_idem (s:concrete_st)
-  : Lemma (ensures eq (merge s s s) s) = ()
-
-(* 2 op Comm  *)
-///////////////////
-
-#set-options "--z3rlimit 300 --ifuel 3"
-let comm_ind_right (l a b c:concrete_st) (o1 o2 o2':op_t)
-  : Lemma (requires Either? (rc o1 o2) /\ 
-                    distinct_ops o1 o2 /\ distinct_ops o1 o2' /\ distinct_ops o2 o2' /\
-                    eq (merge l (do a o1) (do b o2)) (do (do (merge l a b) o2) o1) /\
-                    (Fst_then_snd? (rc o2' o1) ==> (eq (merge l (do a o1) (do b o2')) (do (merge l a (do b o2')) o1))) /\
-                   // ~ (exists o3 a'. eq (do a o1) (do a' o3) /\ distinct_ops o2 o3 /\ Fst_then_snd? (rc o2 o3)) /\
-                    ~ (Fst_then_snd? (rc o1 o2')) )
-                    //~ (exists o3 b'. eq (do (do b o2') o2) (do b' o3) /\ distinct_ops o1 o3 /\ Fst_then_snd? (rc o1 o3)) /\
-                    //~ (exists o3 b'. eq (do b o2) (do b' o3) /\ distinct_ops o1 o3 /\ Fst_then_snd? (rc o1 o3)))                    
-          (ensures eq (merge l (do a o1) (do (do b o2') o2)) (do (do (merge l a (do b o2')) o2) o1)) =   ()
-
-#set-options "--z3rlimit 400 --ifuel 4"
-let comm_ind_left (l a b c:concrete_st) (o1 o2 o1':op_t)
-  : Lemma (requires Either? (rc o1 o2) /\ 
-                    distinct_ops o1 o2 /\ distinct_ops o1 o1' /\ distinct_ops o2 o1' /\
-                    eq (merge l (do a o1) (do b o2)) (do (do (merge l a b) o2) o1) /\
-                    (Fst_then_snd? (rc o1' o2) ==> (eq (merge l (do a o1') (do b o2)) (do (merge l (do a o1') b) o2))) /\
-                    //~ (exists o3 a'. eq (do a o1) (do a' o3) /\ distinct_ops o2 o3 /\ Fst_then_snd? (rc o2 o3)) /\
-                    ~ (Fst_then_snd? (rc o2 o1')) )
-                    //~ (exists o3 b'. eq (do (do b o1') o2) (do b' o3) /\ distinct_ops o1 o3 /\ Fst_then_snd? (rc o1 o3)) /\
-                    //~ (exists o3 b'. eq (do b o2) (do b' o3) /\ distinct_ops o1 o3 /\ Fst_then_snd? (rc o1 o3)))                    
-          (ensures eq (merge l (do (do a o1') o1) (do b o2)) (do (do (merge l (do a o1') b) o2) o1)) = ()
-
-let comm_ind_lca (l:concrete_st) (o1 o2 ol:op_t)
-  : Lemma (requires Either? (rc o1 o2) /\ 
-                    distinct_ops o1 o2 /\ distinct_ops o1 ol /\ distinct_ops o2 ol /\
-                    eq (merge l (do l o1) (do l o2)) (do (do l o2) o1))
-          (ensures eq (merge (do l ol) (do (do l ol) o1) (do (do l ol) o2)) (do (do (do l ol) o2) o1)) = ()
-
-let comm_base (o1 o2:op_t)
-  : Lemma (requires Either? (rc o1 o2) /\ distinct_ops o1 o2)
-          (ensures eq (merge (init_st Ctr_t) (do (init_st Ctr_t) o1) (do (init_st Ctr_t) o2)) (do (do (init_st Ctr_t) o1) o2)) = ()
-
-let comm_base1 (o1 o2:op_t)
-  : Lemma (requires Either? (rc o1 o2) /\ distinct_ops o1 o2)
-          (ensures eq (merge (init_st Gset_t) (do (init_st Gset_t) o1) (do (init_st Gset_t) o2)) (do (do (init_st Gset_t) o1) o2)) = ()
-          
-let comm_inter_base_right (l a b c:concrete_st) (o1 o2 ob ol:op_t) 
-  : Lemma (requires Either? (rc o1 o2) /\ Fst_then_snd? (rc ob ol) /\ 
-                    distinct_ops o1 o2 /\ distinct_ops o1 ob /\ distinct_ops o1 ol /\ distinct_ops o2 ob /\ distinct_ops o2 ol /\ distinct_ops ob ol /\
-                    eq (merge (do l ol) (do (do a ol) o1) (do (do b ol) o2)) (do (do (do c ol) o1) o2) /\ 
-                    eq (merge l (do a o1) (do b o2)) (do (do c o1) o2) /\
-                    eq (merge l (do a o1) (do (do b ob) o2)) (do (do (merge l a (do b ob)) o1) o2) /\ //comes from comm_ind_right
-                    eq (merge (do l ol) (do a ol) (do (do b ob) ol)) (do (do c ob) ol)) //comes from intermediate_base_zero_op
-          (ensures eq (merge (do l ol) (do (do a ol) o1) (do (do (do b ob) ol) o2)) (do (do (do (do c ob) ol) o1) o2)) = ()
-
-let comm_inter_base_left (l a b c:concrete_st) (o1 o2 ob ol:op_t) 
-  : Lemma (requires Either? (rc o1 o2) /\ Fst_then_snd? (rc ob ol) /\ 
-                    distinct_ops o1 o2 /\ distinct_ops o1 ob /\ distinct_ops o1 ol /\ distinct_ops o2 ob /\ distinct_ops o2 ol /\ distinct_ops ob ol /\
-                    eq (merge (do l ol) (do (do a ol) o1) (do (do b ol) o2)) (do (do (do c ol) o1) o2) /\ 
-                    eq (merge l (do a o1) (do b o2)) (do (do c o1) o2) /\
-                    eq (merge l (do (do a ob) o1) (do b o2)) (do (do (merge l (do a ob) b) o1) o2) /\ //comes from comm_ind_left
-                    eq (merge (do l ol) (do (do a ob) ol) (do b ol)) (do (do c ob) ol)) //comes from intermediate_base_zero_op
-          (ensures eq (merge (do l ol) (do (do (do a ob) ol) o1) (do (do b ol) o2)) (do (do (do (do c ob) ol) o1) o2)) = ()
-
-let comm_inter_right (l a b c:concrete_st) (o1 o2 ob ol o:op_t)
-  : Lemma (requires Either? (rc o1 o2) /\ Fst_then_snd? (rc ob ol) /\ 
-                    distinct_ops o1 o2 /\ distinct_ops o1 ob /\ distinct_ops o1 ol /\ distinct_ops o1 o /\ distinct_ops o2 ob /\ 
-                    distinct_ops o2 ol /\ distinct_ops o2 o /\ distinct_ops ob ol /\ distinct_ops ob o /\ distinct_ops ol o /\
-                    get_rid o <> get_rid ol (*o,ol must be concurrent*) /\
-                    //Either? (rc o ol) /\ 
-                    ((~ (commutes_with o ob)) \/ Fst_then_snd? (rc o ol)) /\
-                    eq (merge (do l ol) (do (do a ol) o1) (do (do (do b ob) ol) o2)) (do (do (do (do c ob) ol) o1) o2))
-          (ensures eq (merge (do l ol) (do (do a ol) o1) (do (do (do (do b o) ob) ol) o2)) (do (do (do (do (do c o) ob) ol) o1) o2)) = ()
-
-let comm_inter_left (l a b c:concrete_st) (o1 o2 ob ol o:op_t)
-  : Lemma (requires Either? (rc o1 o2) /\ Fst_then_snd? (rc ob ol) /\ 
-                    distinct_ops o1 o2 /\ distinct_ops o1 ob /\ distinct_ops o1 ol /\ distinct_ops o1 o /\ distinct_ops o2 ob /\ 
-                    distinct_ops o2 ol /\ distinct_ops o2 o /\ distinct_ops ob ol /\ distinct_ops ob o /\ distinct_ops ol o /\
-                    get_rid o <> get_rid ol (*o,ol must be concurrent*) /\
-                    //Either? (rc o ol) /\ 
-                    ((~ (commutes_with o ob)) \/ Fst_then_snd? (rc o ol)) /\
-                    eq (merge (do l ol) (do (do (do a ob) ol) o1) (do (do b ol) o2)) (do (do (do (do c ob) ol) o1) o2))
-          (ensures eq (merge (do l ol) (do (do (do (do a o) ob) ol) o1) (do (do b ol) o2)) (do (do (do (do (do c o) ob) ol) o1) o2)) = ()
-
-let comm_inter_lca (l a b c:concrete_st) (o1 o2 ol:op_t)
-  : Lemma (requires Either? (rc o1 o2) /\ 
-                    distinct_ops o1 o2 /\ distinct_ops o1 ol /\ distinct_ops ol o2 /\
-                    (exists o'. Fst_then_snd? (rc o' ol)) /\
-                    eq (merge l (do a o1) (do b o2)) (do (do c o1) o2))
-          (ensures eq (merge (do l ol) (do (do a ol) o1) (do (do b ol) o2)) (do (do (do c ol) o1) o2)) = ()
-*)
