interface/Dependent_map.fst
@@ -1,0 +1,144 @@
+(*
+   Copyright 2008-2018 Microsoft Research
+
+   Licensed under the Apache License, Version 2.0 (the "License");
+   you may not use this file except in compliance with the License.
+   You may obtain a copy of the License at
+
+       http://www.apache.org/licenses/LICENSE-2.0
+
+   Unless required by applicable law or agreed to in writing, software
+   distributed under the License is distributed on an "AS IS" BASIS,
+   WITHOUT WARRANTIES OR CONDITIONS OF ANY KIND, either express or implied.
+   See the License for the specific language governing permissions and
+   limitations under the License.
+*)
+
+module Dependent_map
+open FStar.Set //Set_extended
+module S = FStar.Set //Set_extended
+open FStar.FunctionalExtensionality
+
+module F = FStar.FunctionalExtensionality
+noeq
+type t (key: eqtype) (value: (key -> Type)) = 
+  { mappings:F.restricted_t key value;
+    domain:S.set key
+  }
+
+let domain (#key: eqtype) (#value: (key -> Tot Type)) (m: t key value) : Tot (S.set key) =
+  m.domain
+  
+let contains (#key: eqtype) (#value: (key -> Tot Type)) (m: t key value) (k: key) : Tot bool =
+  S.mem k m.domain
+
+let sel (#key: eqtype) (#value: (key -> Tot Type)) (m: t key value) (k: key) : Tot (value k) =
+  m.mappings k
+
+let upd (#key: eqtype) (#value: (key -> Tot Type)) (m: t key value) (k: key) (v: value k)
+    : Tot (t key value) =
+  { mappings = F.on_domain key (fun k' -> if k' = k then v else m.mappings k');
+    domain = S.union m.domain (S.singleton k)
+  }
+
+let del(#key: eqtype) (#value: (key -> Tot Type)) (m: t key value) (k: key) : t key value =
+  { mappings = F.on_domain key (fun x -> m.mappings x);
+    domain = S.remove k (domain m)
+  }
+
+let iter_upd (#key:eqtype) (#value1 #value2: (key -> Tot Type)) (f : (k:key) -> value1 k -> value2 k) (m : t key value1) : t key value2 = 
+  { mappings = F.on_domain key (fun x -> f x (m.mappings x));
+    domain =   m.domain
+  }
+
+let create (#key: eqtype) (#value: (key -> Tot Type)) (f: (k: key -> Tot (value k))) : Tot (t key value) = 
+  { mappings = F.on_domain key f;
+    domain = complement empty
+  }
+
+let restrict (#key: eqtype) (#value: (key -> Tot Type)) (s:S.set key) (m: t key value) =
+  { mappings = m.mappings;
+    domain =   S.intersect s m.domain
+  }
+
+let sel_restrict
+      (#key: eqtype)
+      (#value: (key -> Tot Type))
+      (s:S.set key)
+      (m: t key value)
+      (k: key) = ()
+     
+let sel_create (#key: eqtype) (#value: (key -> Tot Type)) (f: (k: key -> Tot (value k))) (k: key)
+    : Lemma (requires True)
+      (ensures (sel #key #value (create f) k == f k))
+      [SMTPat (sel #key #value (create f) k)] = ()
+      
+let sel_upd_same (#key: eqtype) (#value: (key -> Tot Type)) (m: t key value) (k: key) (v: value k) = ()
+
+let sel_upd_other
+      (#key: eqtype)
+      (#value: (key -> Tot Type))
+      (m: t key value)
+      (k: key)
+      (v: value k)
+      (k': key) = ()
+
+let sel_IterUpd (#key:eqtype) (#value1 #value2: (key -> Tot Type)) (f : (k:key) -> value1 k -> value2 k) (m : t key value1) (k:key) = ()
+
+let dom_create (#key: eqtype) (#value: (key -> Tot Type)) (f: (k: key -> Tot (value k))) (k: key) = ()
+
+let dom_upd_same (#key: eqtype) (#value: (key -> Tot Type)) (m: t key value) (k1 k2: key) (v: value k1) = ()
+
+let dom_upd_other (#key: eqtype) (#value: (key -> Tot Type)) (m: t key value) (k1 k2: key) (v: value k2) = ()
+
+let dom_IterUpd (#key:eqtype) (#value1 #value2: (key -> Tot Type)) (f : (k:key) -> value1 k -> value2 k) (m : t key value1) (k:key) = ()
+
+let dom_contains (#key: eqtype) (#value: (key -> Tot Type)) (m: t key value) (k: key) = ()
+
+let lemma_UpdDomain (#key: eqtype) (#value: (key -> Tot Type)) (m: t key value) (k: key) (v: value k) = ()
+
+let dom_restrict (#key: eqtype)
+      (#value: (key -> Tot Type))
+      (s:S.set key)
+      (m: t key value)
+      (k: key)
+      : Lemma (ensures (contains (restrict s m) k == (S.mem k s && contains m k))) = ()
+
+let dom_const_on (#key: eqtype) (#value: (key -> Tot Type)) (k:key) (dom:S.set key) (f: (k:key) -> value k) = ()
+
+let equal (#key: eqtype) (#value: (key -> Tot Type)) (m1 m2: t key value) =
+  F.feq m1.mappings m2.mappings /\
+  S.equal m1.domain m2.domain
+
+let equal_intro (#key: eqtype) (#value: (key -> Tot Type)) (m1 m2: t key value) = ()
+let equal_elim (#key: eqtype) (#value: (key -> Tot Type)) (m1 m2: t key value) = ()
+let equal_refl (#key: eqtype) (#value: (key -> Tot Type)) (m: t key value) = ()
+let equal_intro' (#key: eqtype) (#value: (key -> Tot Type)) (m1 m2: t key value) = ()
+
+let map
+      (#key: eqtype)
+      (#value1 #value2: (key -> Tot Type))
+      (f: (k: key -> value1 k -> Tot (value2 k)))
+      (m: t key value1)
+    : Tot (t key value2) = 
+    { mappings = F.on_domain key (fun k -> f k (sel m k));
+      domain = m.domain }
+
+let sel_map
+      (#key: eqtype)
+      (#value1 #value2: (key -> Tot Type))
+      (f: (k: key -> value1 k -> Tot (value2 k)))
+      (m: t key value1)
+      (k: key)
+     = ()
+
+let map_upd
+      (#key: eqtype)
+      (#value1 #value2: (key -> Tot Type))
+      (f: (k: key -> value1 k -> Tot (value2 k)))
+      (m: t key value1)
+      (k: key)
+      (v: value1 k)
+     = equal_elim #key #value2 (map f (upd m k v)) (upd (map f m) k (f k v))
+
+let dom_map (#key:eqtype) (#value1 #value2: (key -> Tot Type)) (f : (k:key) -> value1 k -> value2 k) (m : t key value1) (k:key) = ()
