interface/Dependent_map.fsti
@@ -1,0 +1,220 @@
+(*
+   Copyright 2008-2018 Microsoft Research
+
+   Licensed under the Apache License, Version 2.0 (the "License");
+   you may not use this file except in compliance with the License.
+   You may obtain a copy of the License at
+
+       http://www.apache.org/licenses/LICENSE-2.0
+
+   Unless required by applicable law or agreed to in writing, software
+   distributed under the License is distributed on an "AS IS" BASIS,
+   WITHOUT WARRANTIES OR CONDITIONS OF ANY KIND, either express or implied.
+   See the License for the specific language governing permissions and
+   limitations under the License.
+*)
+
+module Dependent_map
+module S = FStar.Set //Set_extended
+
+/// This module provides an abstract type of maps whose co-domain
+/// depends on the value of each key. i.e., it is an encapsulation
+/// of [x:key -> value x], where [key] supports decidable equality.
+///
+/// The main constructors of the type are:
+///   * [create]: To create the whole map from a function
+///   * [upd]: To update a map at a point
+///   * [restrict]: To restrict the domain of a map
+///   * [concat]: To concatenate maps by taking the union of their key spaces
+///   * [rename]: To rename the keys of a map
+///   * [map]: To map a function over the values of a map
+///
+/// The main eliminators are:
+///   * [sel]: To query the map for its value at a point
+///
+/// The interface is specified in a style that describes the action of
+/// each eliminator over each of the constructors
+///
+/// The map also supports an extensional equality principle.
+
+(** Abstract type of dependent maps, with universe polymorphic values
+    and keys in universe 0 with decidable equality *)
+val t (key: eqtype) ([@@@strictly_positive] value: (key -> Type u#v)) : Type u#v
+
+(* domain m : The set of keys on which this partial map is defined *)
+val domain(#key: eqtype) (#value: (key -> Tot Type)) (m: t key value) : Tot (S.set key)
+
+(* contains m k: Decides if key `k` is in the map `m` *)
+val contains (#key: eqtype) (#value: (key -> Tot Type)) (m: t key value) (k:key) : Tot bool
+
+(** Querying the map for its value at a given key *)
+val sel (#key: eqtype) (#value: (key -> Tot Type)) (m: t key value) (k: key) : Tot (value k)
+
+(** Updating a map at a point *)
+val upd (#key: eqtype) (#value: (key -> Tot Type)) (m: t key value) (k: key) (v: value k)
+    : Tot (t key value)
+
+(* del m k : A map identical to `m` except the key `k`*)
+val del (#key: eqtype) (#value: (key -> Tot Type)) (m: t key value) (k: key) : Tot (t key value)
+
+val iter_upd (#key:eqtype) (#value1 #value2: (key -> Tot Type)) (f : (k:key) -> value1 k -> value2 k) (m : t key value1) : t key value2
+
+(** Creating a new map from a function *)
+val create (#key: eqtype) (#value: (key -> Tot Type)) (f: (k: key -> Tot (value k)))
+    : Tot (t key value)
+
+(** Restricts the domain of the map to those keys satisfying [p] *)
+val restrict (#key: eqtype) (#value: (key -> Tot Type)) (s:S.set key) (m: t key value) : Tot (t key value)
+
+(** The action of [sel] on [restrict] : the contents of the map isn't changed *)
+val sel_restrict
+      (#key: eqtype)
+      (#value: (key -> Tot Type))
+      (s:S.set key)
+      (m: t key value)
+      (k: key)
+    : Lemma (ensures (sel (restrict s m) k == sel m k))
+
+let const_on (#key:eqtype) (#value: (key -> Tot Type)) (dom:S.set key) (f: (k:key) -> value k) : t key value
+  = restrict dom (create f)
+  
+(** Relating [create] to [sel] *)
+val sel_create (#key: eqtype) (#value: (key -> Tot Type)) (f: (k: key -> Tot (value k))) (k: key)
+    : Lemma (ensures (sel #key #value (create f) k == f k)) [SMTPat (sel #key #value (create f) k)]
+    
+(** The action of selecting a key [k] a map with an updated value [v]
+    at [k]
+
+    This is one of the classic McCarthy select/update axioms in the
+    setting of a dependent map.
+    *)
+val sel_upd_same (#key: eqtype) (#value: (key -> Tot Type)) (m: t key value) (k: key) (v: value k)
+    : Lemma (ensures (sel (upd m k v) k == v)) [SMTPat (sel (upd m k v) k)]
+
+(** The action of selecting a key [k] a map with an updated value [v]
+    at a different key [k']
+
+    This is one of the classic McCarthy select/update axioms in the
+    setting of a dependent map.
+    *)
+val sel_upd_other
+      (#key: eqtype)
+      (#value: (key -> Tot Type))
+      (m: t key value)
+      (k: key)
+      (v: value k)
+      (k': key)
+    : Lemma (requires (k' <> k))
+      (ensures (sel (upd m k v) k' == sel m k'))
+      [SMTPat (sel (upd m k v) k')]
+
+val sel_IterUpd (#key:eqtype) (#value1 #value2: (key -> Tot Type)) (f : (k:key) -> value1 k -> value2 k) (m : t key value1) (k:key)
+  : Lemma (ensures (sel (iter_upd f m) k == f k (sel m k)))
+          [SMTPat (sel (iter_upd f m) k)]
+
+val dom_create (#key: eqtype) (#value: (key -> Tot Type)) (f: (k: key -> Tot (value k))) (k: key)
+  : Lemma (requires True) 
+          (ensures (contains (create f) k))
+          [SMTPat (contains (create f) k)]
+                         
+val dom_upd_same (#key: eqtype) (#value: (key -> Tot Type)) (m: t key value) (k1 k2: key) (v: value k1)
+  : Lemma (requires True) 
+          (ensures (contains (upd m k1 v) k2 == (k1=k2 || contains m k2)))
+          [SMTPat (contains (upd m k1 v) k2)]
+
+val dom_upd_other (#key: eqtype) (#value: (key -> Tot Type)) (m: t key value) (k1 k2: key) (v: value k2)
+  : Lemma (requires True) 
+          (ensures (k2=!=k1 ==> contains (upd m k2 v) k1 == contains m k1))
+          [SMTPat (contains (upd m k2 v) k1)]
+
+val dom_IterUpd (#key:eqtype) (#value1 #value2: (key -> Tot Type)) (f : (k:key) -> value1 k -> value2 k) (m : t key value1) (k:key)
+  : Lemma (ensures (contains (iter_upd f m) k == contains m k))
+          [SMTPat (contains (iter_upd f m) k)]
+
+val dom_contains (#key: eqtype) (#value: (key -> Tot Type)) (m: t key value) (k: key)
+  : Lemma (requires True) 
+          (ensures (contains m k = S.mem k (domain m)))
+          [SMTPatOr[[SMTPat (contains m k)]; [SMTPat (S.mem k (domain m))]]]
+
+val lemma_UpdDomain (#key: eqtype) (#value: (key -> Tot Type)) (m: t key value) (k: key) (v: value k)
+  : Lemma (requires True)
+          (ensures (S.equal (domain (upd m k v)) (S.union (domain m) (S.singleton k))))
+          [SMTPat (domain (upd m k v))]
+
+val dom_restrict (#key: eqtype)
+      (#value: (key -> Tot Type))
+      (s:S.set key)
+      (m: t key value)
+      (k: key)
+      : Lemma (ensures (contains (restrict s m) k == (S.mem k s && contains m k)))
+              [SMTPat (contains (restrict s m) k)]
+
+val dom_const_on (#key: eqtype) (#value: (key -> Tot Type)) (k:key) (dom:S.set key) (f: (k:key) -> value k)
+  : Lemma (requires True) 
+          (ensures (contains (const_on dom f) k = S.mem k dom))
+          [SMTPat (contains (const_on dom f) k)]
+          
+(** Extensional propositional equality on maps *)
+val equal (#key: eqtype) (#value: (key -> Tot Type)) (m1 m2: t key value) : prop
+
+(** Introducing extensional equality by lifting equality on the map, pointwise *)
+val equal_intro (#key: eqtype) (#value: (key -> Tot Type)) (m1 m2: t key value)
+    : Lemma (requires (forall k. sel m1 k == sel m2 k /\ contains m1 k = contains m2 k))
+      (ensures (equal m1 m2))
+      [SMTPat (equal m1 m2)]
+
+val equal_elim (#key: eqtype) (#value: (key -> Tot Type)) (m1 m2: t key value)
+  : Lemma (ensures (equal m1 m2 <==> m1 == m2))
+          [SMTPat (m1 == m2)]
+                            
+(** [equal] is reflexive *)
+val equal_refl (#key: eqtype) (#value: (key -> Tot Type)) (m: t key value)
+    : Lemma (ensures (equal m m)) [SMTPat (equal m m)]
+
+val equal_intro' (#key: eqtype) (#value: (key -> Tot Type)) (m1 m2: t key value)
+  : Lemma (requires (equal m1 m2))
+          (ensures (forall k. sel m1 k == sel m2 k /\ contains m1 k = contains m2 k))
+          [SMTPat (equal m1 m2)]
+                                            
+(** [equal] can be eliminated into standard propositional equality
+    (==), also proving that it is an equivalence relation *)
+//val equal_elim (#key: eqtype) (#value: (key -> Tot Type)) (m1 m2: t key value)
+  //  : Lemma (requires (equal m1 m2)) (ensures (m1 == m2)) [SMTPat (equal m1 m2)]
+
+(**** Mapping a function over a dependent map *)
+
+(** [map f m] applies f to each value in [m]'s co-domain *)
+val map
+      (#key: eqtype)
+      (#value1 #value2: (key -> Tot Type))
+      (f: (k: key -> value1 k -> Tot (value2 k)))
+      (m: t key value1)
+    : Tot (t key value2)
+
+(** The action of [sel] on [map] *)
+val sel_map
+      (#key: eqtype)
+      (#value1 #value2: (key -> Tot Type))
+      (f: (k: key -> value1 k -> Tot (value2 k)))
+      (m: t key value1)
+      (k: key)
+    : Lemma (ensures (sel (map f m) k == f k (sel m k)))
+      [SMTPat (sel #key #value2 (map #key #value1 #value2 f m) k)]
+
+(** [map] explained in terms of its action on [upd] *)
+val map_upd
+      (#key: eqtype)
+      (#value1 #value2: (key -> Tot Type))
+      (f: (k: key -> value1 k -> Tot (value2 k)))
+      (m: t key value1)
+      (k: key)
+      (v: value1 k)
+    : Lemma (ensures (map f (upd m k v) == upd (map f m) k (f k v)))
+      [
+        //AR: wanted to write an SMTPatOr, but gives some error
+        SMTPat (map #key #value1 #value2 f (upd #key #value1 m k v))
+      ]
+
+val dom_map (#key:eqtype) (#value1 #value2: (key -> Tot Type)) (f : (k:key) -> value1 k -> value2 k) (m : t key value1) (k:key)
+  : Lemma (ensures (contains (map f m) k == contains m k))
+          [SMTPat (contains (map f m) k)]
